Arithmetic: refactor using sections
- factorize call semantics
- simplify program semantics (no args passed)
- use custom inductive principle for statements
- rename Notations.v into Prelude.v and set some options
- remove external expression semantics (was unused)

Arithmetic/theories/Languages/MiniC/Facts.v
@@ -1,121 +1,144 @@
 From Coq Require Import FinFun.
+From RecordUpdate Require Import RecordUpdate.
+From Equations Require Import Equations.
 From RAC Require Import Utils Environnement.
 From RAC.Languages Require Import Syntax MiniC.Semantics.
 
 Import FunctionalEnv Domain Facts.
 
-Fact untouched_var_same_eval_exp {T : Set} : forall exp_sem, 
-    _untouched_var_same_eval_exp exp_sem ->
-    _untouched_var_same_eval_exp (@generic_exp_sem T exp_sem).
-Proof with eauto with rac_hint.
-    intros exp_sem Hext ev e v x Hnotin Hderiv. induction Hderiv ; simpl in Hnotin...
-    - split... constructor. simpl. apply p_map_not_same_eq... StringSet.D.fsetdec.
-    - split ; 
-        intro x';  econstructor...
-        + apply IHHderiv1. StringSet.D.fsetdec. 
-        + apply IHHderiv2. StringSet.D.fsetdec.
-        + apply IHHderiv1... StringSet.D.fsetdec. 
-        + apply IHHderiv2... StringSet.D.fsetdec. 
-    - split;
-        intro x';  econstructor...
-        + apply IHHderiv1... StringSet.D.fsetdec. 
-        + apply IHHderiv2... StringSet.D.fsetdec. 
-        + apply IHHderiv1... StringSet.D.fsetdec. 
-        + apply IHHderiv2... StringSet.D.fsetdec. 
-    - split ; 
-        intro x';  econstructor...
-        + apply IHHderiv1... StringSet.D.fsetdec. 
-        + apply IHHderiv2... StringSet.D.fsetdec.  
-        + apply IHHderiv1... StringSet.D.fsetdec. 
-        + apply IHHderiv2... StringSet.D.fsetdec.  
-Qed.
 
-Fact untouched_var_same_eval_stmt {S T : Set} : 
-    forall exp_sem stmt_sem ext_stmt_vars, 
-    _untouched_var_same_eval_stmt exp_sem stmt_sem ext_stmt_vars ->
-    _untouched_var_same_eval_stmt exp_sem (@generic_stmt_sem S T exp_sem stmt_sem ext_stmt_vars) ext_stmt_vars.
-Proof with auto with rac_hint.
-    intros exp_sem stmt_sem ext_stmt_vars Hext f ev ev' s x Hderiv [Hnotin Huservar]. induction Hderiv ; simpl in Hnotin; trivial.
-    - simpl. autounfold with rac_hint. rewrite p_map_not_same... StringSet.D.fsetdec.
-    -  apply IHHderiv. StringSet.D.fsetdec.
-    - apply IHHderiv. StringSet.D.fsetdec. 
-    - apply IHHderiv.  simpl. StringSet.D.fsetdec.
-    - destruct IHHderiv.
-        + StringSet.D.fsetdec.
-        + apply IHHderiv0. StringSet.D.fsetdec. 
-    - simpl. symmetry. apply p_map_not_same_eq... StringSet.D.fsetdec.
-    (* return *)
-    - simpl. destruct (eq_dec res_f x). subst. 
-        * discriminate.
-        * autounfold with rac_hint. symmetry...
-    - eapply Hext in H...
-Qed.
+Section GenericFacts.
+    Context {S T : Set} {ext_stmt_vars : S -> StringSet.t} {fe : @fenv S T}.
+    
+    Variable (stmt_sem : forall f e, @generic_stmt_sem_sig S T f e).
 
-Fact determinist_exp_eval {T : Set}: 
-forall ext_exp_sem, _determinist_exp_eval ext_exp_sem -> _determinist_exp_eval (@generic_exp_sem T ext_exp_sem).
-Proof.
-    intros ext_exp_sem ext_inj. unfold _determinist_exp_eval. intros e. induction e ; intros ; inversion H ; inversion H0 ; subst ; try easy.
-    4,5:
-        apply IHe1 with (v:=VInt (z ⁱⁿᵗ z_ir)) (v':=VInt (z0 ⁱⁿᵗ z_ir0)) in H11 ; [|assumption] ; injection H11 as eqz ;
-        apply IHe2 with (v:=VInt (z' ⁱⁿᵗ z'_ir)) (v':= VInt (z'0 ⁱⁿᵗ z'_ir0)) in H13; [|assumption] ;  injection H13 as eqz' ; subst ; now rewrite H14 in H7.
-    - f_equal. f_equal. now apply Int.mi_eq. 
-    - congruence.
-    - f_equal. f_equal. apply Int.mi_eq. simpl. f_equal.
-        + apply IHe1 with (v:=VInt (z ⁱⁿᵗ z_ir)) (v':= VInt (z0 ⁱⁿᵗ z_ir0)) in H13; [|assumption]. now injection H13. 
-        + apply IHe2 with (v:=VInt (z' ⁱⁿᵗ z'_ir)) (v':=VInt (z'0 ⁱⁿᵗ z'_ir0)) in H14; [|assumption]. now injection H14.
-Qed.
+    Notation generic_exp_sem := (fun e => @generic_exp_sem T e).
+    Notation generic_stmt_sem := (fun f e => @generic_stmt_sem _ _ stmt_sem ext_stmt_vars f e).
 
 
-Fact _determinist_c_exp_eval {T} : _determinist_exp_eval (@Empty_exp_sem T).
-Proof. easy. Qed.
+    Fact untouched_var_same_eval_exp : 
+        @_untouched_var_same_eval_exp T generic_exp_sem.
+    Proof with eauto with rac_hint.
+        clear stmt_sem fe.
+        intros ev e v x Hnotin Hderiv.  induction Hderiv ; simpl in Hnotin...
+        - split ; constructor...  intros. simpl. apply p_map_not_same_eq... StringSet.D.fsetdec.
+        - split ; 
+            intro x';  econstructor...
+            + apply IHHderiv1. StringSet.D.fsetdec. 
+            + apply IHHderiv2. StringSet.D.fsetdec.
+            + apply IHHderiv1... StringSet.D.fsetdec. 
+            + apply IHHderiv2... StringSet.D.fsetdec. 
+        - split;
+            intro x';  econstructor...
+            + apply IHHderiv1... StringSet.D.fsetdec. 
+            + apply IHHderiv2... StringSet.D.fsetdec. 
+            + apply IHHderiv1... StringSet.D.fsetdec. 
+            + apply IHHderiv2... StringSet.D.fsetdec. 
+        - split ; 
+            intro x';  econstructor...
+            + apply IHHderiv1... StringSet.D.fsetdec. 
+            + apply IHHderiv2... StringSet.D.fsetdec. 
+            + apply IHHderiv1... StringSet.D.fsetdec. 
+            + apply IHHderiv2... StringSet.D.fsetdec.  
+    Qed.
 
-Definition determinist_c_exp_eval {T}:= determinist_exp_eval (@Empty_exp_sem T) _determinist_c_exp_eval.
+    Fact untouched_var_same_eval_stmt : 
+        @_untouched_var_same_eval_stmt _ _ stmt_sem ext_stmt_vars fe ->
+        @_untouched_var_same_eval_stmt _ _ generic_stmt_sem ext_stmt_vars fe.
+    Proof with auto with rac_hint.
+        intros Hext ev ev' s x Hderiv [Hnotin Huservar]. induction Hderiv ; simpl in Hnotin; trivial.
+        - simpl. autounfold with rac_hint. rewrite p_map_not_same... StringSet.D.fsetdec.
+        -  apply IHHderiv. StringSet.D.fsetdec.
+        - apply IHHderiv. StringSet.D.fsetdec. 
+        - apply IHHderiv.  simpl. StringSet.D.fsetdec.
+        - destruct IHHderiv1.
+            + StringSet.D.fsetdec.
+            + apply IHHderiv2. StringSet.D.fsetdec. 
+        - simpl. symmetry. apply p_map_not_same_eq... StringSet.D.fsetdec.
+        (* return *)
+        - simpl. destruct (eq_dec res_f x).
+            + subst. discriminate.
+            + autounfold with rac_hint. symmetry...
+        - eapply Hext in H...
+    Qed.
 
-Fact Forall2_same_zargs { T : Set} : forall ev eargs zargs zargs0  exp_sem, 
-    _determinist_exp_eval exp_sem
-    -> List.Forall2 (@generic_exp_sem T exp_sem ev) eargs zargs 
-    -> List.Forall2 (@generic_exp_sem T exp_sem ev) eargs zargs0 -> zargs = zargs0.
-Proof.
-    intros ev eargs zargs zargs0 exp H  Hderiv. generalize dependent zargs0. induction Hderiv ; intros zargs0 H1.
-    - now inversion H1.
-    - destruct zargs0. inversion H1. apply List.Forall2_cons_iff in H1 as [H1 Hderiv2].
-        apply determinist_exp_eval in H0 ; [|assumption]. apply H0 in H1. subst. f_equal. clear H0.
-        now apply IHHderiv in Hderiv2.
-Qed.
+    Fact determinist_exp_eval : 
+        _determinist_exp_eval generic_exp_sem.
+    Proof.
+        intros e. induction e ; intros ; inversion H ; inversion H0 ; subst ; try easy.
+        4,5:
+            apply IHe1 with (v:=VInt (z ⁱⁿᵗ z_ir)) (v':=VInt (z0 ⁱⁿᵗ z_ir0)) in H11 ; [|assumption] ; injection H11 as eqz ;
+            apply IHe2 with (v:=VInt (z' ⁱⁿᵗ z'_ir)) (v':= VInt (z'0 ⁱⁿᵗ z'_ir0)) in H13; [|assumption] ;  injection H13 as eqz' ; subst ; now rewrite H14 in H7.
+        - f_equal. f_equal. now apply Int.mi_eq. 
+        - congruence.
+        - f_equal. f_equal. apply Int.mi_eq. simpl. f_equal.
+            + apply IHe1 with (v:=VInt (z ⁱⁿᵗ z_ir)) (v':= VInt (z0 ⁱⁿᵗ z_ir0)) in H13; [|assumption]. now injection H13. 
+            + apply IHe2 with (v:=VInt (z' ⁱⁿᵗ z'_ir)) (v':=VInt (z'0 ⁱⁿᵗ z'_ir0)) in H14; [|assumption]. now injection H14.
+    Qed.
 
-Fact determinist_stmt_eval {S T : Set}: 
-    forall ext_exp_sem ext_stmt_sem ext_stmt_vars, 
-    @_determinist_stmt_eval S T ext_exp_sem ext_stmt_sem -> 
-    _determinist_stmt_eval ext_exp_sem (@generic_stmt_sem S T ext_exp_sem ext_stmt_sem ext_stmt_vars).
-Proof with auto. 
-    intros ext_exp_sem ext_stmt_sem ext_stmt_vars Hds Hde f s ev ev' Hderiv. induction Hderiv ; intros.
-    - inversion H... 
-    - inversion H2 ; subst... repeat f_equal.  apply determinist_exp_eval in H8... specialize (H8 z). apply H8 in H1. now inversion H1.
-    - inversion H1 ; subst...  apply determinist_exp_eval in H6... destruct H as [H []]. apply H6 in H. now inversion H.
-    - inversion H1 ; subst... apply determinist_exp_eval in H... destruct H6 as [H2 []]. apply H in H2. now inversion H2.
-    - inversion H0... 
-    - inversion H1 ; subst... apply IHHderiv in H4. subst. apply IHHderiv0 in H6. now subst. 
-    - inversion H5 ; subst. 
-       (* same args, same body *) 
-            rewrite H10 in H0. injection H0 as H0. subst.
+
+    (* Definition determinist_c_exp_eval := @determinist_exp_eval Empty_exp_sem _determinist_c_exp_eval. *)
+
+    Fact Forall2_same_zargs : 
+        forall ev eargs zargs zargs0, 
+        List.Forall2 (generic_exp_sem ev) eargs zargs 
+        -> List.Forall2 (generic_exp_sem ev) eargs zargs0 
+        -> zargs = zargs0.
+    Proof.
+        intros ev eargs zargs zargs0 Hderiv. generalize dependent zargs0. induction Hderiv ; intros zargs0 H1.
+        - now inversion H1.
+        - destruct zargs0; [inversion H1|].
+            apply List.Forall2_cons_iff in H1 as [H1 Hderiv2].
+            apply determinist_exp_eval in H1.  apply H1 in H. subst. f_equal. clear H1.
+            now apply IHHderiv in Hderiv2.
+    Qed.
+
+    Fact determinist_stmt_eval : 
+        _determinist_stmt_eval generic_exp_sem stmt_sem (fe:=fe) -> 
+        _determinist_stmt_eval generic_exp_sem generic_stmt_sem (fe:=fe).
+    Proof with auto.
+        intros  Hds Hde s ev ev' Hderiv. induction Hderiv using @generic_stmt_sem_full_ind; intros.
+
+        - inversion H...    
+        - inversion_clear H2... repeat f_equal.  apply determinist_exp_eval in H5... specialize (H5 z). apply H5 in H1. now inversion H1. 
+        - inversion_clear H0...  apply determinist_exp_eval in H1... destruct H as [H []]. apply H1 in H. now inversion H.
+        - inversion_clear H0... exfalso.  apply determinist_exp_eval in H... destruct H1 as [H1 Hnotz]. apply H in H1. inversion H1. now apply Hnotz.
+        - inversion H... 
+        - inversion_clear H... apply IHHderiv1 in H0. subst. apply IHHderiv2 in H1. now subst. 
+        - inversion_clear H4. destruct H5 as (Hl & Hf & Hargs & Hsem).
+            (* same args, same body *) 
+            assert (Heq: xargs = xargs0 /\ b = b0) by (rewrite Hf in H0; now inversion_clear H0). inversion_clear Heq. subst.
             (* same args eval *) 
             assert (zargs = zargs0). {
-                pose proof (@Forall2_same_zargs T ev eargs vargs vargs0 ext_exp_sem Hde H1 H11) as H0. unfold vargs,vargs0 in H0.
-                apply list_map_id_eq in H0. assumption. unfold Injective. intros x y H7. now inversion H7. 
+                pose proof (Forall2_same_zargs _ _ _ _  H1 Hargs) as Hsame.
+                apply list_map_id_eq in Hsame; [assumption|]. unfold Injective. intros x y Heq. now inversion Heq. 
             }
-            subst. apply IHHderiv in H12. subst. rewrite H4 in H15. injection H15 as H15. now subst.
-    - inversion H3.  subst.  rewrite H7 in H0. injection H0 as Eq1. subst. 
-             assert (zargs = zargs0). {
-                pose proof (@Forall2_same_zargs T ev eargs vargs vargs0 ext_exp_sem Hde H1 H8) as H0. unfold vargs,vargs0 in H0.
-                apply list_map_id_eq in H0. assumption. unfold Injective. intros x y Heq. now inversion Heq. 
-             }
-             subst.
-            apply IHHderiv in H10. now subst.
-    - inversion H0 ; subst... apply determinist_exp_eval in H... apply H in H2. injection H2 as H2. now subst.
-    - inversion H1...
-    - inversion H0. subst. unfold _determinist_stmt_eval in Hds. eapply Hds... apply H. apply H2.
-Qed.
+            subst. apply IHHderiv in Hsem. subst. rewrite H7 in H3. injection H3 as H3. now subst.
 
-Fact _determinist_c_stmt_eval {S T} : @_determinist_stmt_eval S T Empty_exp_sem Empty_stmt_sem. easy. Qed.
-Definition determinist_c_stmt_eval {S T} := determinist_stmt_eval Empty_exp_sem Empty_stmt_sem Empty_ext_stmt_vars (@_determinist_c_stmt_eval S T).
+                
+        - inversion_clear H2. destruct H3 as (Hl & Hf & Hargs & Hsem). 
+            assert (Heq: xargs = xargs0 /\ b = b0) by (rewrite Hf in H0; now inversion_clear H0). inversion_clear Heq. subst.
+            assert (zargs = zargs0). {
+                pose proof (@Forall2_same_zargs  _ _ _ _ H1 Hargs) as Hsame. 
+                apply list_map_id_eq in Hsame ; [assumption|]. unfold Injective. intros x y Heq. now inversion Heq. 
+            }
+            subst. apply IHHderiv in Hsem. now subst.
+        - inversion H0 ; subst... apply determinist_exp_eval in H... apply H in H2. injection H2 as H2. now subst.
+        - inversion H1...
+        - inversion H0. subst. unfold _determinist_stmt_eval in Hds. eapply Hds...
+            + apply H.
+            + apply H2. 
+    Qed.
 
+End GenericFacts.
+
+
+Fact _determinist_c_exp_eval {T : Set} : @_determinist_exp_eval T Empty_exp_sem.
+Proof. easy. Qed.
+
+Fact _determinist_c_stmt_eval {S T : Set} {ext_stmt_vars} : 
+    @_determinist_stmt_eval S T Empty_exp_sem Empty_stmt_sem ext_stmt_vars.
+Proof. easy. Qed.
+
+
+(* Definition determinist_c_stmt_eval {S T } fe := @determinist_stmt_eval S T Empty_ext_stmt_vars fe Empty_stmt_sem  _determinist_c_stmt_eval. *)
