Arithmetic/theories/Languages/MiniC/Semantics.v
@@ -1,4 +1,4 @@
-From Coq Require Import Strings.String ZArith.ZArith.
+From Coq Require Import Strings.String ZArith.ZArith Sets.Ensembles.
 From RecordUpdate Require Import RecordUpdate.
 From RAC Require Import Utils Environnement.
 From RAC.Languages Require Import Syntax.
@@ -18,217 +18,405 @@ Declare Scope generic_exp_sem_scope.
 Delimit Scope generic_exp_sem_scope with gesem.
 
 
+#[local] Open Scope utils_scope.
+#[local] Open Scope mini_c_scope.
+
+
+Import FunctionalEnv Domain.
+
+
 Definition compiler_prefix : id := "_".
 Definition comp_var x : id  := (compiler_prefix ++ x)%string.
 Definition is_comp_var := String.prefix compiler_prefix.
 Definition res_f : id := comp_var "res".
 
-Definition exp_sem_sig {T : Set} : Type := Env -> @_c_exp T -> 𝕍 -> Prop.
-Definition stmt_sem_sig {S T: Set} : Type  :=  @fenv S T -> Env -> @_c_statement S T ->  Env -> Prop.
-Definition Empty_exp_sem {T: Set} : @exp_sem_sig T := fun _ _ _ => False.
-Definition Empty_stmt_sem {S T: Set} : @stmt_sem_sig S T := fun _ _ _ _ => False.
 
 
+Section GenericSemantics.
+    Context {F S T : Set}.
 
-(* extensible expression semantic *)
-Inductive generic_exp_sem {T:Set} {ext_exp : @exp_sem_sig T} (ev:Env): @_c_exp T -> 𝕍 -> Prop :=
-| C_E_Int (z:Z) irz : ev |= z => VInt (z ⁱⁿᵗ irz)
-| C_E_Var (x:𝓥) z : 
-    ev x = Some (Def (VInt z)) -> 
-    ev |=  (C_Id x C_Int) => z
-| C_E_BinOpInt e e' (z z':Z) op z_ir z'_ir
-    (H:Int.inRange (⋄ op z z')) :
-    ev |= e =>  VInt (z ⁱⁿᵗ z_ir) ->
-    ev |= e' =>  VInt (z' ⁱⁿᵗ z'_ir) ->
-    ev |=  BinOpInt e op e' => VInt ((⋄ op) z z' ⁱⁿᵗ H)
-| C_E_BinOpTrue e e' (z z' : Z) z_ir z'_ir op :
-    ev |= e => VInt (z ⁱⁿᵗ z_ir) ->
-    ev |= e' => VInt (z' ⁱⁿᵗ z'_ir) ->
-    (◁ op) z z' = true ->
-    ev |= BinOpBool e op e' => VInt one
-| C_E_BinOpFalse e e' (z z' : Z) op z_ir z'_ir :
-    ev |= e => VInt (z ⁱⁿᵗ z_ir) -> 
-    ev |= e' => VInt (z' ⁱⁿᵗ z'_ir) -> 
-    ((◁ op) z z' = false ) ->
-    ev |= BinOpBool e op e' => VInt zero
-(* | C_Ext x v t: 
-    (* variable must not be of type int (treated by C_E_Var) *)
-    t <> C_Int ->
+    Notation c_type      := (@c_type T).
+    Notation c_exp       := (@c_exp T).
+    Notation c_statement := (@c_statement S T).
+    Notation c_decl      := (@c_decl T).
+    Notation c_routine   := (@c_routine F S T).
+    Notation c_program   := (@c_program F S T).
+    Notation fenv        := (@fenv S T).
+
+    Definition generic_exp_sem_sig  (_:Env) : Type := c_exp -> 𝕍 -> Prop.
+    Definition generic_stmt_sem_sig  (_:fenv) (_:Env) : Type := c_statement -> Env -> Prop.
+
+    Definition Empty_exp_sem e : generic_exp_sem_sig e := fun _ _ => False.
+    Definition Empty_stmt_sem f e : generic_stmt_sem_sig f e := fun _ _ => False.
+
+    Variable (ext_exp_sem : forall e, generic_exp_sem_sig e) (ext_stmt_sem : forall f e, generic_stmt_sem_sig f e).
     
-    (* variable must be bound and init *)
-    ev x = Some (Def v) ->
+    Variable (rel : Env -> Env -> Prop).
+    Variable (rel_s : Env -> Env -> σ -> Prop).
+
+    Context {ext_stmt_vars : S -> StringSet.t} {ext_ty_val: 𝕍 -> c_type} .
+
+    Section FunctionsEnv.
+
+        Context {fe: fenv}.
+
+        (* extensible expression semantic *)
+        Inductive generic_exp_sem ev : generic_exp_sem_sig ev :=
+        | C_E_Int (z:Z) irz : ev |= z => VInt (z ⁱⁿᵗ irz)
+
+        | C_E_Var (x:𝓥) z : 
+            ev x = Some (Def (VInt z)) -> 
+            ev |=  (C_Id x C_Int) => z
+
+        | C_E_BinOpInt e e' (z z':Z) op z_ir z'_ir
+            (H:Int.inRange (⋄ op z z')) :
+            ev |= e =>  VInt (z ⁱⁿᵗ z_ir) ->
+            ev |= e' =>  VInt (z' ⁱⁿᵗ z'_ir) ->
+            ev |=  BinOpInt e op e' => VInt ((⋄ op) z z' ⁱⁿᵗ H)
+
+        | C_E_BinOpTrue e e' (z z' : Z) z_ir z'_ir op :
+            ev |= e => VInt (z ⁱⁿᵗ z_ir) ->
+            ev |= e' => VInt (z' ⁱⁿᵗ z'_ir) ->
+            (◁ op) z z' = true ->
+            ev |= BinOpBool e op e' => VInt one
+
+        | C_E_BinOpFalse e e' (z z' : Z) op z_ir z'_ir :
+            ev |= e => VInt (z ⁱⁿᵗ z_ir) -> 
+            ev |= e' => VInt (z' ⁱⁿᵗ z'_ir) -> 
+            ((◁ op) z z' = false ) ->
+            ev |= BinOpBool e op e' => VInt zero
+
+        (* | C_Ext x v t: 
+            (* variable must not be of type int (treated by C_E_Var) *)
+            t <> C_Int ->
+            
+            (* variable must be bound and init *)
+            ev x = Some (Def v) ->
 
 
-    (* the external semantic can only add additional constraint, the result is always v *)
-    ext_exp ev (C_Id x t) v ->
+            (* the external semantic can only add additional constraint, the result is always v *)
+            ext_exp ev (C_Id x t) v ->
 
-    ev |= (C_Id x t) => v *)
+            ev |= (C_Id x t) => v *)
 
-where  "env '|=' e => z" := (generic_exp_sem env e z) : generic_exp_sem_scope.
-#[global] Hint Constructors generic_exp_sem  : rac_hint.
+        where  "env '|=' e => z" := (generic_exp_sem env e z) : generic_exp_sem_scope.
+        
 
-Definition c_exp_sem := @generic_exp_sem Empty_set Empty_exp_sem.
-Notation "Ω '|=' e => v"  := (c_exp_sem Ω e v) : c_sem_scope.
+        Definition generic_call_sem  
+            {g_exp_s : forall e, generic_exp_sem_sig e}
+            {g_stmt_s : forall e, generic_stmt_sem_sig fe e}
+            (prj: fenv -> _)  (ev body_init_env:Env) name xargs eargs zargs b b_ev :=
 
-#[local] Open Scope utils_scope.
-#[local] Open Scope mini_c_scope.
-Import FunctionalEnv.
-
-(* extensible statement semantic *)
-Inductive generic_stmt_sem {S T: Set} {ext_exp: @exp_sem_sig T} {ext_stmt: @stmt_sem_sig S T} {ext_stmt_vars:  S -> StringSet.t} (f : @fenv S T) (ev:Env) : @_c_statement S T -> Env -> Prop := 
-    | S_skip  :  (ev |= <{ skip }> => ev) f
-    | S_Assign x (z: Int.MI) (e : @_c_exp T) : 
-        (* must not be a compiler variable i.e. function return value *)
-        is_comp_var x = false ->
-
-        type_of_value (ev x) = Some C_Int ->
-        @generic_exp_sem T ext_exp ev e z -> 
-        (ev |= <{(Assign x e)}> => (ev <| env ; vars ::= {{x\Def z}} |>)) f
-
-    | S_IfTrue ev' (z : Int.MI) e s s' :
-        @generic_exp_sem T ext_exp ev e z /\ ~ (z = VInt zero) ->
-        (ev  |= s => ev') f ->
-        (ev  |= <{ if e s else s'}> => ev') f
-
-    | S_IfFalse ev' e s s' :
-        @generic_exp_sem T ext_exp ev e (VInt zero) ->
-        (ev |= s' => ev') f ->
-        (ev |= <{ if e s else s'}> => ev') f
-
-    | S_While e s  ev' :
-        (ev |= <{ if e s ; while e s else skip }> => ev') f ->
-        (ev |= <{ while e s }> => ev') f
-
-    | S_Seq  ev' ev'' s s' :
-        (ev |= s => ev') f ->
-        (ev' |= s' => ev'') f ->
-        (ev |= <{ s ; s' }> =>  ev'') f
-
-    | S_FCall fname (b: @_c_statement S T) b_ev c xargs eargs (zargs : Int.MI*) z : 
-        List.length xargs = List.length eargs ->
-        let vargs := List.map (fun x => Def (VInt x)) zargs in 
-        StringMap.find fname f.(funs) = Some (xargs,b) ->
-        List.Forall2 (@generic_exp_sem T ext_exp ev) eargs vargs ->
-        (empty_env <| env ; vars ::= p_map_addall_back xargs vargs |> |= b => b_ev) f -> 
-        ~ StringSet.In res_f (stmt_vars b ext_stmt_vars) -> 
-        b_ev res_f = Some (Def (VInt z)) -> (* must be a defined integer value *)
-        (ev |= (FCall c fname eargs) => ev <| env ; vars ::= {{c\Def z}} |> <| mstate := b_ev |>) f
-
-    | S_PCall p b ev' xargs eargs (zargs : Int.MI*) : 
-        List.length xargs = List.length eargs ->
-        let vargs := List.map (fun x => Def (VInt x)) zargs  in 
-        StringMap.find p f.(procs)  = Some (xargs,b) ->
-        List.Forall2 (@generic_exp_sem T ext_exp ev) eargs vargs ->
-        (empty_env <| env ; vars ::= p_map_addall_back xargs vargs |> |= b => ev') f -> 
-        (ev |= PCall p eargs => ev <| mstate := ev' |>) f
-
-    | S_Return e (z: Int.MI) : 
-        @generic_exp_sem T ext_exp ev e (Def (VInt z)) ->
-        (ev |= <{ return e }> => ev <| env ; vars ::= {{res_f\Def (VInt z)}} |>) f
-
-    | S_PAssert e (z: Int.MI) :
-        @generic_exp_sem T ext_exp ev e z -> z <> VInt zero ->
-        (ev |= <{ assert e }> => ev) f
-
-    | S_ExtSem s ev' :  
-        (* only S_Ext constructor allowed to use external semantic*)
-        ext_stmt f ev (S_Ext s) ev' 
-        -> (ev |= (S_Ext s) => ev') f
-    
-    where "env |= s => env'"  := (fun f => generic_stmt_sem f env s env') : generic_stmt_sem_scope.
-#[global] Hint Constructors generic_stmt_sem  : rac_hint.
+            List.length xargs = List.length eargs /\
+            let vargs := List.map (fun x => Def (VInt x)) zargs in 
+            StringMap.find name (prj fe) = Some (xargs,b) /\
+            List.Forall2 (g_exp_s ev) eargs vargs /\
+            g_stmt_s (body_init_env <| env ; vars ::= p_map_addall_back xargs vargs |>) b b_ev.
 
 
+        (* extensible statement semantic *)
+        Inductive generic_stmt_sem ev : generic_stmt_sem_sig fe ev := 
 
-Inductive generic_decl_sem {T} {ext_ty_val: 𝕍 -> @_c_type T} (ev:Env) : @_c_decl T -> Env -> Prop :=
-| D_Decl x (t:@_c_type T) u:
-    ev.(vars) x  = None -> 
-    _type_of_value ext_ty_val (Some (Undef u)) = Some t  ->
-    generic_decl_sem ev (C_Decl t x) (ev <| env ;vars ::= {{x\Undef u}} |>)
-.
+        | S_Skip  :  (ev |= <{ skip }> => ev)
+        | S_Assign x (z: Int.MI) (e : c_exp) : 
+            (* must not be a compiler variable i.e. function return value *)
+            is_comp_var x = false ->
+
+            type_of_value (ev x) = Some C_Int ->
+            generic_exp_sem ev e z -> 
+            ev |= <{(Assign x e)}> => (ev <| env ; vars ::= {{x\Def z}} |>)
+
+        | S_IfTrue ev' (z : Int.MI) e s s' :
+            generic_exp_sem ev e z /\ ~ (z = VInt zero) ->
+            ev  |= s => ev' ->
+            ev  |= <{ if e s else s'}> => ev'
+
+        | S_IfFalse ev' e s s' :
+            @generic_exp_sem ev e (VInt zero) ->
+            ev |= s' => ev' ->
+            ev |= <{ if e s else s'}> => ev'
+
+        | S_While e s  ev' :
+            ev |= <{ if e s ; while e s else skip }> => ev' ->
+            ev |= <{ while e s }> => ev'
+
+        | S_Seq  ev' ev'' s s' :
+            ev |= s => ev' ->
+            ev' |= s' => ev'' ->
+            ev |= <{ s ; s' }> =>  ev''
+
+        | S_FCall fname b b_ev xargs eargs (zargs : Int.MI*) c z : 
+            @generic_call_sem generic_exp_sem generic_stmt_sem 
+            funs ev empty_env fname xargs eargs zargs b b_ev ->
+
+            ~ StringSet.In res_f (stmt_vars b ext_stmt_vars) -> 
+            b_ev res_f = Some (Def (VInt z)) -> (* must be a defined integer value *)
+            ev |= FCall c fname eargs => ev <| env ; vars ::= {{c\Def z}} |> <| mstate := b_ev |>
+
+        | S_PCall pname b b_ev xargs eargs (zargs : Int.MI*) : 
+            @generic_call_sem generic_exp_sem generic_stmt_sem
+            procs ev empty_env pname xargs eargs zargs b b_ev ->
+
+            ev |= PCall pname eargs => ev <| mstate := b_ev |>
+
+        | S_Return e (z: Int.MI) : 
+            generic_exp_sem ev e (Def (VInt z)) ->
+            ev |= <{ return e }> => ev <| env ; vars ::= {{res_f\Def (VInt z)}} |>
+
+        | S_PAssert e (z: Int.MI) :
+            generic_exp_sem ev e z -> z <> VInt zero ->
+            ev |= <{ assert e }> => ev
+
+        | S_ExtSem s ev' :  
+            (* only S_Ext constructor allowed to use external semantic*)
+            ext_stmt_sem fe ev (S_Ext s) ev' 
+            -> ev |= (S_Ext s) => ev'
+
+        where "env |= s => env'"  := (generic_stmt_sem env s env') : generic_stmt_sem_scope.
 
 
-From Coq Require Import Sets.Ensembles.
+        Section Induction.
+
+        Variable P :  Env -> c_statement -> Env -> Prop.
+        Variable P1 : forall ev, P ev <{skip}> ev.
+        Variable P2 : forall (ev : Env) (x : id) (z : Int.MI) (e : c_exp),
+            is_comp_var x = false ->
+            type_of_value (ev x) = Some C_Int ->
+            (ev |= e => z)%gesem ->
+            P ev (Assign x e) (ev <| env; vars ::= {{x \Def z}} |>)
+        .
+
+        Variable P3 : forall (ev ev' : Env) (z : Int.MI) (e : c_exp) (s : c_statement) (s' : Syntax.c_statement),
+            (ev |= e => z)%gesem /\ z <> zero ->
+            (ev |= s => ev')%gssem -> P ev s ev' -> P ev <{if e s else s'}> ev'
+        .
+        Variable P4 : forall (ev ev' : Env) (e : c_exp) (s s' : c_statement),
+            (ev |= e => zero)%gesem ->
+            (ev |= s' => ev')%gssem -> P ev s' ev' -> P ev <{if e s else s'}> ev'
+        .
+        Variable P5 :  forall (ev : Env) (e : c_exp) (s : c_statement) (ev' : Env),
+            (ev |= <{if e s; while e s else skip}> => ev')%gssem ->
+            P ev <{if e s; while e s else skip}> ev' -> P ev <{while e s}> ev'
+        .
+        Variable P6 : forall (ev ev' ev'' : Env) (s s' : c_statement),
+            (ev |= s => ev')%gssem ->
+            P ev s ev' ->
+            (ev' |= s' => ev'')%gssem -> 
+            P ev' s' ev'' -> 
+            P ev <{s; s'}> ev''
+        .
+        Variable P7 : forall (ev : Env) (fname : StringMap.key) (b : c_statement) (b_ev : Env) (xargs : 𝓥 *) (eargs : c_exp *) (zargs : Int.MI *) (c : id)  (z : Int.MI),
+            (* inlining of generic_call_sem *)
+            List.length xargs = List.length eargs ->
+            let vargs := List.map (fun x => Def (VInt x)) zargs in 
+            StringMap.find fname fe.(funs) = Some (xargs,b) ->
+            List.Forall2 (generic_exp_sem ev) eargs vargs ->
+            generic_stmt_sem (empty_env <| env ; vars ::= p_map_addall_back xargs vargs |>) b b_ev ->
+            P  (empty_env <| env ; vars ::= p_map_addall_back xargs vargs |>) b b_ev ->
+            ~ StringSet.In res_f (stmt_vars b ext_stmt_vars) ->
+            b_ev res_f = Some (Def z) ->
+            P ev (FCall c fname eargs) (ev <| env; vars ::= {{c \Def z}} |> <| mstate := b_ev |>)
+        .
+        Variable P8 : forall (ev : Env) (pname : StringMap.key) 
+          (b : c_statement) (b_ev : Env) (xargs : 𝓥 *) 
+          (eargs : c_exp *) (zargs : Int.MI *),
+            (* inlining of generic_call_sem *)
+            List.length xargs = List.length eargs ->
+            let vargs := List.map (fun x => Def (VInt x)) zargs in 
+            StringMap.find pname fe.(procs) = Some (xargs,b) ->
+            List.Forall2 (generic_exp_sem ev) eargs vargs ->
+            generic_stmt_sem (empty_env <| env ; vars ::= p_map_addall_back xargs vargs |>) b b_ev ->
+            P (empty_env <| env ; vars ::= p_map_addall_back xargs vargs |>) b b_ev ->
+            P ev (PCall pname eargs) (ev <| mstate := b_ev |>)
+        .
+
+        Variable P9 : forall (ev : Env) (e : c_exp) (z : Int.MI),
+            (ev |= e => z)%gesem ->
+            P ev <{return e}> (ev <| env; vars ::= {{res_f \Def z}} |>)
+        .
+        Variable P10 : forall (ev : Env) (e : c_exp) (z : Int.MI),
+        (ev |= e => z)%gesem -> z <> zero -> P ev <{assert e}> ev
+        .
+        Variable P11 : forall (ev : Env) (s : S) (ev' : Env),
+            ext_stmt_sem fe ev (S_Ext s) ev' -> P ev (S_Ext s) ev'
+        .
+
+
+        Fixpoint generic_stmt_sem_full_ind  ev s ev' (sem : (ev |= s => ev')%gssem) : P ev s ev' := match sem with
+        | S_Skip _ => P1 ev
+        | S_Assign _ x z Hcomp Hty Hesem Hsem => P2 ev x z Hcomp Hty Hesem Hsem
+        | S_IfTrue _ ev' z e0 s s' a g0 => P3 ev ev' z e0 s s' a g0 (generic_stmt_sem_full_ind ev s ev' g0)
+        | S_IfFalse _ ev' e0 s s' g0 g1 => P4 ev ev' e0 s s' g0 g1 (generic_stmt_sem_full_ind ev s' ev' g1)
+        | S_While _ e0 s ev' g0 => P5 ev e0 s ev' g0 (generic_stmt_sem_full_ind ev <{if e0  s; while e0 s else  skip}> ev' g0)
+        | S_Seq _ ev' ev'' s s' g0 g1 => P6 ev ev' ev'' s s' g0 (generic_stmt_sem_full_ind ev s ev' g0) g1 (generic_stmt_sem_full_ind ev' s' ev'' g1)
+        | S_FCall _ fname b b_ev xargs eargs zargs c0 z (conj H1 (conj H2 (conj H3 H4))) n e0 => 
+            let vargs := List.map (fun x => Def (VInt x)) zargs in
+            P7 ev fname b b_ev xargs eargs zargs c0 z H1 H2 H3 H4 (generic_stmt_sem_full_ind (empty_env <| env ; vars ::= p_map_addall_back xargs vargs |>) b b_ev H4) n e0
+        | S_PCall _ pname b b_ev xargs eargs zargs (conj H1 (conj H2 (conj H3 H4))) => 
+            let vargs := List.map (fun x => Def (VInt x)) zargs in
+            P8 ev pname b b_ev xargs eargs zargs H1 H2 H3 H4 (generic_stmt_sem_full_ind (empty_env <| env ; vars ::= p_map_addall_back xargs vargs |>) b b_ev H4)
+        | S_Return _ e0 z g0 => P9 ev e0 z g0
+        | S_PAssert _ e0 z g0 n => P10 ev e0 z g0 n
+        | S_ExtSem _ s ev' s0 => P11 ev s ev' s0
+        end
+        .
+        End Induction.
 
 
 
-Inductive declare_vars {T} {ext_ty_val: 𝕍 -> @_c_type T} (e : Env) : Ensemble (@_c_decl T) -> Env -> Prop :=
-| DV_nil : 
-    declare_vars e (Empty_set _) e
-
-| DV_cons decls d e': 
-    @generic_decl_sem T ext_ty_val e d e' -> 
-    declare_vars e (Add _ decls d) e'
-.
+        Inductive generic_decl_sem  (ev:Env) : c_decl -> Env -> Prop :=
+        | D_Decl x (t: c_type) u:
+            ev.(vars) x  = None -> 
+            _type_of_value ext_ty_val (Some (Undef u)) = Some t ->
+            generic_decl_sem ev (C_Decl t x) (ev <| env ;vars ::= {{x\Undef u}} |>)
+        .
 
 
 
+        Inductive declare_vars (e : Env) : Ensemble c_decl -> Env -> Prop :=
+        | DV_nil : 
+            declare_vars e (Empty_set _) e
 
-Inductive generic_pgrm_sem {F S T:Set} 
-    {ext_ty_val: 𝕍 -> @_c_type T} {ext_exp : @exp_sem_sig T} {ext_stmt: @stmt_sem_sig S T} {ext_stmt_vars: S -> StringSet.t} 
-    {build_fenv : @_c_routine F S T * -> @fenv S T}
-    (ev:Env) (P : @_c_program F S T) (args:Int.MI* ) : Env -> Prop :=
+        | DV_cons decls d e': 
+            generic_decl_sem e d e' -> 
+            declare_vars e (Add _ decls d) e'
+        .
 
-    | P_Pgrm params b ret z ev_decls  ev':
+
+
+        Definition _untouched_var_same_eval_exp : Prop := 
+            forall (ev:Env) e v x,
+            ~ StringSet.In v (exp_vars e) -> 
+            generic_exp_sem ev e x ->
+            (forall x', ext_exp_sem (ev <| env ; vars ::= {{v\x'}} |>)  e x)
+            /\ 
+            (forall l z', 
+            no_aliasing ev ->
+            ev v = Some (Def (VMpz (Some l))) -> generic_exp_sem (ev <| mstate ::= {{l\z'}} |>) e x)
+        .
+
+        Definition _untouched_var_same_eval_stmt : Prop := 
+            forall ev ev' s x, 
+            ext_stmt_sem fe ev s ev' ->
+            ~ StringSet.In x (stmt_vars s ext_stmt_vars) /\ is_comp_var x = false -> 
+            ev x = ev' x
+        .
+
+        Definition _no_mem_aliasing : Prop := 
+            forall (ev:Env) s (ev':Env), 
+            no_aliasing ev
+            -> ext_stmt_sem fe ev s ev' 
+            -> no_aliasing ev'
+        .
+
+        Definition _determinist_exp_eval : Prop := 
+            forall e ev v, ext_exp_sem ev e v ->  
+            forall v', ext_exp_sem ev e v' -> v = v'
+        .
+
+
+        Definition _determinist_stmt_eval : Prop := 
+            _determinist_exp_eval -> 
+            forall s ev ev',  ext_stmt_sem fe ev s ev' ->  
+            forall ev'', ext_stmt_sem fe ev s ev'' -> ev' = ev''
+        .
+
+        Definition _LC1_weakening_of_expression_semantics : Prop := 
+            forall e ev (x:𝕍), 
+            ext_exp_sem ev e x <-> (forall ev', rel ev ev' -> ext_exp_sem ev' e x)
+        .
+
+        Definition _LC21_weakening_of_statement_semantics : Prop := 
+            (*
+            should be in both directions according to the article but right to left does not work :
+            We will see if the 'bad' direction is used in the proof 
+            If this is the cast, one direction is trying to add to have a new env_01 = ev_0 + a and a new env_02 = ev_0 + b so that 
+                (ev0 + a) inter ev0 + b) = ev1
+            *)  
+            _LC1_weakening_of_expression_semantics  ->
+            forall ev₀ s ev₁,
+            ext_stmt_sem fe ev₀ s ev₁ ->
+            ( forall ev₀' sub, rel_s ev₀ ev₀' sub ->
+                exists ev₁', 
+                rel_s ev₁ ev₁' sub /\ ext_stmt_sem fe ev₀' s ev₁')
+        .
+
+        Definition _LC22_weakening_of_statement_semantics : Prop := 
+            _LC1_weakening_of_expression_semantics ->
+            forall ev₀ ev₀' s ev₁ sub,
+            ext_stmt_sem fe ev₀ s ev₁ /\ rel_s ev₀ ev₀' sub  ->
+            (
+                forall ev₁',
+                ext_stmt_sem fe ev₀' s ev₁'->
+                (* if v is a compiler variable, i.e. a function return value, v can change*)
+                (forall (v:𝓥), (v ∉ ev₀) /\ is_comp_var v = false  -> ev₀' v = ev₁' v)%dom_
+                /\
+                (forall (x:location), (forall v, ev₀ v <> Some (Def (VMpz x))) -> ev₀'.(mstate) (proj1_sig sub x) = ev₁'.(mstate) (proj1_sig sub x))
+            )
+        .
+
+        (* required to prove _LC23_weakening_of_statement_semantics *)
+        Definition _LC1_weakening_of_expression_semantics_3 : Prop := 
+            forall ev e z sub,
+            ext_exp_sem ev e z ->
+            
+            forall ev', rel_s ev' ev sub ->
+            (
+                (forall v, (dom ev - dom ev') v -> ~ StringSet.In v (exp_vars e))
+                /\
+                (forall x, (dom ev.(mstate) - dom ev'.(mstate)) x -> (exists v, ev v = Some (induced (proj1_sig sub) (Def (VMpz x))) /\ ~ StringSet.In v (exp_vars e)))
+            )%dom_ ->
+
+            ext_exp_sem  ev' e z
+        .
+
+        Definition _LC23_weakening_of_statement_semantics : Prop := 
+            forall ev₀  s ev₁ sub,
+            ext_stmt_sem fe ev₀ s ev₁ -> 
+
+            forall ev₀', rel_s ev₀' ev₀ sub ->
+            (
+                (forall v, (dom ev₀ - dom ev₀') v -> ~ StringSet.In v (stmt_vars s ext_stmt_vars))
+                /\
+                (
+                    forall x, (dom ev₀.(mstate) - dom ev₀'.(mstate)) x -> 
+                    (exists v, ev₀ v = Some (induced (proj1_sig sub) (Def (VMpz x))) 
+                    /\ ~ StringSet.In v (stmt_vars s ext_stmt_vars))
+                )
+            )%dom_ ->
+
+            exists ev₁', ext_stmt_sem fe ev₀' s ev₁'
+        .
+
+    End FunctionsEnv.
+
+    Inductive generic_pgrm_sem {build_fenv : @c_routine* -> fenv} (ev:Env) (P : c_program) : Env -> Prop :=
+
+    | P_Pgrm b z ev_decls b_ev:
 
         (* add global declarations to the env *)
-        @declare_vars T ext_ty_val ev (list_to_ensemble (fst P)) ev_decls ->
+        declare_vars ev (list_to_ensemble (fst P)) ev_decls ->
+
         (* add all functions to fenv *)
-        let fenv := build_fenv (snd P) in
+        let fe := build_fenv (snd P) in
 
-        (* call the main function with the given parameters (same as F_Call except the evaluation env for the body is not empty and we keep the env from the body) *) 
-        let vargs := List.map (fun x => Def (VInt x)) args in 
-        StringMap.find "main"%string fenv.(funs) = Some (params,b) ->
-        List.length params = List.length vargs ->
-        @generic_stmt_sem S T ext_exp ext_stmt ext_stmt_vars fenv (ev_decls <| env ; vars ::= p_map_addall_back params vargs |>)  b ev' -> 
+        (** call the main function with the given parameters 
+            (same as function call except the evaluation env for the body is not initially empty and we keep the whole final env) 
+        *) 
+        @generic_call_sem fe generic_exp_sem (fun e => @generic_stmt_sem fe e)
+        funs ev ev_decls "main"%string nil nil nil b b_ev ->
+
+
         ~ StringSet.In res_f (stmt_vars b ext_stmt_vars) -> 
-        ev' res_f = Some (Def (VInt z)) -> (* must be a defined integer value *)
+        b_ev res_f = Some (Def (VInt z)) -> (* must return a defined integer value *)
+        generic_pgrm_sem ev P b_ev
+    .
 
-        generic_pgrm_sem ev P args (ev' <| env; vars ::= {{ret\Def z}} |>)
-.
-
-
-Definition _untouched_var_same_eval_exp {T : Set} (exp_sem : @exp_sem_sig T) := 
-    forall (ev:Env) (e: @_c_exp T) v x,
-    ~ StringSet.In v (exp_vars e) -> 
-    exp_sem ev e x ->
-    (forall x', exp_sem (ev <| env ; vars ::= {{v\x'}} |>)  e x)
-    /\ 
-    (forall l z', 
-    no_aliasing ev ->
-    ev v = Some (Def (VMpz (Some l))) -> exp_sem (ev <| mstate ::= {{l\z'}} |>) e x).
+End GenericSemantics.
 
 
-
-Definition _untouched_var_same_eval_stmt {S T : Set} (exp_sem : @exp_sem_sig T) (stmt_sem : @stmt_sem_sig S T) (ext_stmt_vars : S -> StringSet.t) := 
-    forall f ev ev' (s: @_c_statement S T) x, 
-    stmt_sem f ev s ev' ->
-    ~ StringSet.In x (stmt_vars s ext_stmt_vars) /\ is_comp_var x = false -> 
-    ev x = ev' x
-.
-
-Definition _no_mem_aliasing {S T : Set} (stmt_sem : @stmt_sem_sig S T)  : Prop := 
-    forall (exp_sem:@exp_sem_sig T) f (ev:Env) s (ev':Env), 
-    no_aliasing ev
-    -> stmt_sem f ev s ev' 
-    -> no_aliasing ev'.
-
-
-Definition _determinist_exp_eval {T : Set} (exp_sem : @exp_sem_sig T) : Prop := 
-forall e ev v,  exp_sem ev e v ->  (forall v', exp_sem ev e v' -> v = v')
-.
-
-
-Definition _determinist_stmt_eval {S T : Set} (ext_exp_sem : @exp_sem_sig T) (stmt_sem : @stmt_sem_sig S T) : Prop := 
-    @_determinist_exp_eval T ext_exp_sem  -> 
-    forall f s ev ev',  stmt_sem f ev s ev' ->  (forall ev'', stmt_sem f ev s ev'' -> ev' = ev'').
-
-Definition _LC1_weakening_of_expression_semantics {T} (exp_sem : @exp_sem_sig T) (rel: Env -> Env -> Prop): Prop := 
-    forall e ev (x:𝕍), 
-    exp_sem ev e x <-> (forall ev', rel ev ev' -> exp_sem ev' e x).
-
-
-Fact weakening_of_empty_expression_semantics {T} : _LC1_weakening_of_expression_semantics (@Empty_exp_sem T) exist_env_mem_partial_order. 
+Fact weakening_of_empty_expression_semantics {T} : 
+    @_LC1_weakening_of_expression_semantics T (@Empty_exp_sem T) exist_env_mem_partial_order. 
 Proof.
     unfold _LC1_weakening_of_expression_semantics. intros. split ; unfold Empty_exp_sem.
     - intros [].
@@ -236,91 +424,37 @@ Proof.
 Qed.
 
 
-
-Definition _LC21_weakening_of_expression_semantics  {S T : Set} (exp_sem : @exp_sem_sig T) (stmt_sem : @stmt_sem_sig S T) 
-    (rel: Env -> Env -> σ -> Prop) := 
-    (*
-    should be in both directions according to the article but right to left does not work :
-    We will see if the 'bad' direction is used in the proof 
-    If this is the cast, one direction is trying to add to have a new env_01 = ev_0 + a and a new env_02 = ev_0 + b so that 
-        (ev0 + a) inter ev0 + b) = ev1
-    *)  
-    _LC1_weakening_of_expression_semantics exp_sem (fun e e' => existify (rel e e')) ->
-    forall (f : @fenv S T) ev₀ s ev₁,
-    stmt_sem f ev₀ s ev₁ ->
-    ( forall ev₀' sub, rel ev₀ ev₀' sub ->
-        exists ev₁', 
-        rel ev₁ ev₁' sub /\ stmt_sem f ev₀' s ev₁').
-
-Fact weakening_of_empty_statement_semantics_1 {S T}: forall rel, _LC21_weakening_of_expression_semantics (@Empty_exp_sem T) (@Empty_stmt_sem S T) rel.
-Proof. 
+Fact weakening_of_empty_statement_semantics_1 {S T} rel rel_s f exp_sem:
+    @_LC21_weakening_of_statement_semantics S T exp_sem (@Empty_stmt_sem S T) rel rel_s f.
+Proof.
     easy. 
 Qed.
 
-Import Domain.
 
-Definition _LC22_weakening_of_expression_semantics  {S T : Set} (exp_sem : @exp_sem_sig T) (stmt_sem : @stmt_sem_sig S T) 
-    (rel: Env -> Env -> σ -> Prop)
-    := 
-    _determinist_exp_eval exp_sem ->
-    _LC1_weakening_of_expression_semantics exp_sem (fun e e' => existify (rel e e')) ->
-    forall (f: @fenv S T) ev₀ ev₀' s ev₁ sub,
-    stmt_sem f ev₀ s ev₁ /\ rel ev₀ ev₀' sub  ->
-    (
-        forall ev₁',
-        stmt_sem f ev₀' s ev₁'->
-        (* if v is a compiler variable, i.e. a function return value, v can change*)
-        (forall (v:𝓥), (v ∉ ev₀) /\ is_comp_var v = false  -> ev₀' v = ev₁' v)%dom_
-        /\
-        (forall (x:location), (forall v, ev₀ v <> Some (Def (VMpz x))) -> ev₀'.(mstate) (proj1_sig sub x) = ev₁'.(mstate) (proj1_sig sub x))
-    ).
-
-
-Fact weakening_of_empty_statement_semantics_2 {S T}: forall rel, _LC22_weakening_of_expression_semantics (@Empty_exp_sem T) (@Empty_stmt_sem S T) rel.
+Fact weakening_of_empty_statement_semantics_2 {S T} rel rel_s f exp_sem: 
+    @_LC22_weakening_of_statement_semantics S T exp_sem (@Empty_stmt_sem S T) rel rel_s f.
 Proof. 
     easy. 
 Qed.
 
 
-(* required to prove _LC23_weakening_of_expression_semantics *)
-Definition _LC1_weakening_of_expression_semantics_3 {T : Set} (exp_sem : @exp_sem_sig T)  (rel: Env -> Env -> σ -> Prop) := 
-    forall ev e z sub,
-    exp_sem ev e z ->
-    
-    forall ev', rel ev' ev sub ->
-    (
-        (forall v, (dom ev - dom ev') v -> ~ StringSet.In v (exp_vars e))
-        /\
-        (forall x, (dom ev.(mstate) - dom ev'.(mstate)) x -> (exists v, ev v = Some (induced (proj1_sig sub) (Def (VMpz x))) /\ ~ StringSet.In v (exp_vars e)))
-    )%dom_ ->
-
-    exp_sem  ev' e z
-.
-
-
-Fact weakening_of_empty_expression_semantics_3 {T}: forall rel, _LC1_weakening_of_expression_semantics_3 (@Empty_exp_sem T) rel.
+Fact weakening_of_empty_expression_semantics_3 {T} rel : 
+    @_LC1_weakening_of_expression_semantics_3 T (@Empty_exp_sem T) rel.
 Proof. 
     easy.
 Qed.
 
 
-
-Definition _LC23_weakening_of_expression_semantics  {S T : Set} (stmt_sem : @stmt_sem_sig S T) (ext_stmt_vars: S -> StringSet.t)
-    (rel: Env -> Env -> σ -> Prop)  := 
-    forall f ev₀  s ev₁ sub,
-    stmt_sem f ev₀ s ev₁ -> 
-
-    forall ev₀', rel ev₀' ev₀ sub ->
-    (
-        (forall v, (dom ev₀ - dom ev₀') v -> ~ StringSet.In v (stmt_vars s ext_stmt_vars))
-        /\
-        (forall x, (dom ev₀.(mstate) - dom ev₀'.(mstate)) x -> (exists v, ev₀ v = Some (induced (proj1_sig sub) (Def (VMpz x))) /\ ~ StringSet.In v (stmt_vars s ext_stmt_vars)))
-    )%dom_ ->
-
-    exists ev₁', stmt_sem f ev₀' s ev₁'
-    .
-
-Fact weakening_of_empty_statement_semantics_3 {S T}: forall f rel, _LC23_weakening_of_expression_semantics (@Empty_stmt_sem S T) f rel.
+Fact weakening_of_empty_statement_semantics_3 {S T} rel rel_s stmt_vars :
+    @_LC23_weakening_of_statement_semantics S T (@Empty_stmt_sem S T)  rel rel_s stmt_vars.
 Proof. 
     easy. 
 Qed.
+
+
+Definition c_exp_sem :=  @generic_exp_sem Datatypes.Empty_set.
+Notation "Ω '|=' e => v"  := (c_exp_sem Ω e v) : c_sem_scope.
+
+
+#[global] Hint Constructors generic_exp_sem : rac_hint.
+#[global] Hint Constructors generic_stmt_sem : rac_hint.
