Arithmetic/theories/Languages/MiniFSL/Semantics.v
@@ -107,7 +107,7 @@ Inductive _fsl_assert_sem  (f : fenv ) (ev:Env) : fsl_statement -> Env -> Prop :
 #[global] Hint Constructors _fsl_assert_sem : rac_hint.
 
 
-Definition fsl_stmt_sem := @generic_stmt_sem _fsl_statement Empty_set Empty_exp_sem _fsl_assert_sem _fsl_stmt_vars.
+Definition fsl_stmt_sem := @generic_stmt_sem _fsl_statement Empty_set _fsl_assert_sem _fsl_stmt_vars.
 
 Declare Scope fsl_sem_scope.
 Delimit Scope fsl_sem_scope with fslsem.
@@ -116,6 +116,6 @@ Notation "ev |= s => ev'"  := (fun f => fsl_stmt_sem f ev s ev') : fsl_sem_scope
 
 
 Definition fsl_pgrm_sem := 
-    @generic_pgrm_sem _fsl_routine _fsl_statement Empty_set (fun _ => Void) Empty_exp_sem _fsl_assert_sem _fsl_stmt_vars build_fsl_fenv. 
+    @generic_pgrm_sem _fsl_routine _fsl_statement Empty_set _fsl_assert_sem _fsl_stmt_vars (fun _ => Void)  build_fsl_fenv    . 
 
 
