Arithmetic/theories/Languages/MiniGMP/Semantics.v
@@ -17,76 +17,110 @@ Delimit Scope gmp_stmt_sem_scope with gmpssem.
 Definition declare_gmp_vars := @declare_vars _gmp_t (fun x => T_Ext Mpz).
 
 
-Inductive _gmp_stmt_sem  (f : rac_prog_fenv) (ev:Env) : gmp_statement -> Env -> Prop := 
-    | S_init x (l:location) u:
-        (forall v, ev v <> Some (Def (VMpz (Some l)))) ->
-        ev x = Some (Undef (UMpz u)) ->
-        (ev |= <(init(x))> => ev <| env ; vars ::= {{x\Def (VMpz (Some l))}} |> <| mstate ::= {{l\Defined 0}} |>) f
-    
-    | S_clear x a u:   
-        ev x = Some (Def (VMpz (Some a))) ->   
-        (ev |= <(cl(x))> => ev <| env ; vars ::= {{x\(Def (VMpz None))}} |> <| mstate ::= {{a\Undefined u}} |>) f
+Section GMPSemantics.
+    Variable (fe: rac_prog_fenv).
 
-    | S_set_i x y z a :  
-        ev x = Some (Def (VMpz (Some a))) ->
-        (ev |= y => VInt z)%csem ->
-        (ev |= <(set_i(x,y))> => ev <| mstate ::= {{a\Defined (z ̇)}} |>) f
+    Inductive _gmp_stmt_sem  (fe:rac_prog_fenv) (ev:Env) :  gmp_statement -> Env -> Prop := 
+        | S_init x (l:location) u:
+            (forall v, ev v <> Some (Def (VMpz (Some l)))) ->
+            ev x = Some (Undef (UMpz u)) ->
+            ev |= <(init(x))> => ev <| env ; vars ::= {{x\Def (VMpz (Some l))}} |> <| mstate ::= {{l\Defined 0}} |>
+        
+        | S_clear x a u:   
+            ev x = Some (Def (VMpz (Some a))) ->   
+            ev |= <(cl(x))> => ev <| env ; vars ::= {{x\(Def (VMpz None))}} |> <| mstate ::= {{a\Undefined u}} |>
 
-    | S_set_z x y z (a n : location) :  
-        ev x = Some (Def (VMpz a)) ->
-        ev y = Some (Def (VMpz n)) ->
-        ev.(mstate) n = Some (Defined z) ->
-        (ev |= <(set_z(x,y))> => ev <| mstate ::= {{a\Defined z}} |>) f 
+        | S_set_i x y z a :  
+            ev x = Some (Def (VMpz (Some a))) ->
+            (ev |= y => VInt z)%csem ->
+            ev |= <(set_i(x,y))> => ev <| mstate ::= {{a\Defined (z ̇)}} |>
 
-    | S_get_int x y ly zy (ir:Int.inRange zy) :
-        ev y = Some (Def (VMpz (Some ly))) ->
-        ev.(mstate) ly = Some (Defined zy) -> 
-        (ev |= <(x = get_int(y))> => ev <| env ; vars ::= {{x\VInt (zy ⁱⁿᵗ ir) : 𝕍}} |>) f
+        | S_set_z x y z (a n : location) :  
+            ev x = Some (Def (VMpz a)) ->
+            ev y = Some (Def (VMpz n)) ->
+            ev.(mstate) n = Some (Defined z) ->
+            ev |= <(set_z(x,y))> => ev <| mstate ::= {{a\Defined z}} |> 
 
-    | S_set_s s x zx lx :
-        ev x = Some (Def (VMpz (Some lx))) ->
-        BinaryString.to_Z s = zx ->
-        (ev |= <(set_s(x,s))> => ev <| mstate ::= {{lx\Defined zx}} |> ) f
+        | S_get_int x y ly zy (ir:Int.inRange zy) :
+            ev y = Some (Def (VMpz (Some ly))) ->
+            ev.(mstate) ly = Some (Defined zy) -> 
+            ev |= <(x = get_int(y))> => ev <| env ; vars ::= {{x\VInt (zy ⁱⁿᵗ ir) : 𝕍}} |>
 
-    | S_cmp c x (lx ly :location) zx y zy (b:𝕍):
-        ev x = Some (Def (VMpz (Some lx))) ->
-        ev y = Some (Def (VMpz (Some ly))) ->
-        ev.(mstate) lx = Some (Defined zx) ->
-        ev.(mstate) ly = Some (Defined zy) ->
-        (
-            (Z.gt zx zy <-> b = VInt one) /\
-            (Z.lt zx zy <-> b = VInt sub_one) /\
-            (Z.eq zx zy <-> b = VInt zero)
-        ) ->
-        (ev |= <(c = cmp(x,y))> => ev <| env ; vars ::= {{c\b}} |>) f
-    
-    | S_op bop r lr x y (lx ly : location) zx zy :
-        ev x = Some (Def (VMpz (Some lx))) ->
-        ev y = Some (Def (VMpz (Some ly))) ->
-        ev.(mstate) lx = Some (Defined zx) ->
-        ev.(mstate) ly = Some (Defined zy) ->
-        ev r = Some (Def (VMpz (Some lr))) -> (* not in paper *)
-        (ev |= fsl_to_gmp_op bop r x y => ev <| mstate ::= {{lr\Defined (⋄ (□ bop) zx zy) }} |>) f
+        | S_set_s s x zx lx :
+            ev x = Some (Def (VMpz (Some lx))) ->
+            BinaryString.to_Z s = zx ->
+            ev |= <(set_s(x,s))> => ev <| mstate ::= {{lx\Defined zx}} |> 
 
-    | S_Scope decls (s:@_c_statement _gmp_statement _gmp_t) ev_s ev_s':
-        (*
-            - A scope has var declarations that gets dropped at the end, except the memory state. 
-            - This was missing in the original paper but required in the translation 
-            as we must create a scope when we translate the assertions 
-            - Note it complicate things because the statement are c instructions, not just gmp ones.
-        *)
-        declare_gmp_vars ev (list_to_ensemble decls) ev_s ->
-        @generic_stmt_sem _gmp_statement _gmp_t Empty_exp_sem _gmp_stmt_sem _gmp_stmt_vars f ev_s s ev_s' -> 
-        (ev |= GMP_Scope decls s =>  ev <| mstate := ev_s' |> ) f
+        | S_cmp c x (lx ly :location) zx y zy (b:𝕍):
+            ev x = Some (Def (VMpz (Some lx))) ->
+            ev y = Some (Def (VMpz (Some ly))) ->
+            ev.(mstate) lx = Some (Defined zx) ->
+            ev.(mstate) ly = Some (Defined zy) ->
+            (
+                (Z.gt zx zy <-> b = VInt one) /\
+                (Z.lt zx zy <-> b = VInt sub_one) /\
+                (Z.eq zx zy <-> b = VInt zero)
+            ) ->
+            ev |= <(c = cmp(x,y))> => ev <| env ; vars ::= {{c\b}} |>
+        
+        | S_op bop r lr x y (lx ly : location) zx zy :
+            ev x = Some (Def (VMpz (Some lx))) ->
+            ev y = Some (Def (VMpz (Some ly))) ->
+            ev.(mstate) lx = Some (Defined zx) ->
+            ev.(mstate) ly = Some (Defined zy) ->
+            ev r = Some (Def (VMpz (Some lr))) -> (* not in paper *)
+            ev |= fsl_to_gmp_op bop r x y => ev <| mstate ::= {{lr\Defined (⋄ (□ bop) zx zy) }} |>
 
-
-where "ev |= s => ev'" := (fun f => _gmp_stmt_sem f ev s ev') : ext_gmp_stmt_sem_scope.
-
-#[global] Hint Constructors _gmp_stmt_sem  : rac_hint.
+        | S_Scope decls (s:@c_statement _gmp_statement _gmp_t) ev_s ev_s':
+            (*
+                - A scope has var declarations that gets dropped at the end, except the memory state. 
+                - This was missing in the original paper but required in the translation 
+                as we must create a scope when we translate the assertions 
+                - Note it complicate things because the statement are c instructions, not just gmp ones.
+            *)
+            declare_gmp_vars ev (list_to_ensemble decls) ev_s ->
+            @generic_stmt_sem _gmp_statement _gmp_t _gmp_stmt_sem _gmp_stmt_vars fe ev_s s ev_s' -> 
+            ev |= GMP_Scope decls s =>  ev <| mstate := ev_s' |>
 
 
-Definition gmp_stmt_sem := @generic_stmt_sem _gmp_statement _gmp_t Empty_exp_sem _gmp_stmt_sem _gmp_stmt_vars.
+    where "ev |= s => ev'" := (_gmp_stmt_sem fe (ev:Env) (s:_gmp_statement) (ev':Env)) : ext_gmp_stmt_sem_scope.
+
+    Section Induction.
+
+        (* Variable P : Env -> 𝐒 -> Env -> Prop.
+        Variable P1 : forall x (l:location) u,
+            (forall v, ev v <> Some (Def (VMpz (Some l)))) ->
+            ev x = Some (Undef (UMpz u)) ->
+            (ev |= <(init(x))> => ev <| env ; vars ::= {{x\Def (VMpz (Some l))}} |> <| mstate ::= {{l\Defined 0}} |>) f
+        .
+        
+        Fixpoint _gmpt_stmt_sem_full_ind f ev s ev' (sem : (ev |= s => ev')%extgmpssem f) : P ev s ev' :=
+        match s in (_gmp_stmt_sem _ _ g0 e0) return (P g0 e0) with
+        | S_init _ _ x l u x0 x1 => P1 x l u x0 x1
+        | S_clear _ _ x a u x0 => P2 x a u x0
+        | S_set_i _ _ x y z a x0 x1 => P3 x y z a x0 x1
+        | S_set_z _ _ x y z a n x0 x1 x2 => P4 x y z a n x0 x1 x2
+        | S_get_int _ _ x y ly zy ir x0 x1 => P5 x y ly zy ir x0 x1
+        | S_set_s _ _ s x zx lx x0 x1 => P6 s x zx lx x0 x1
+        | S_cmp _ _ c x lx ly zx y zy b x0 x1 x2 x3 x4 =>
+            P7 c x lx ly zx y zy b x0 x1 x2 x3 x4
+        | S_op _ _ bop r lr x y lx ly zx zy x0 x1 x2 x3 x4 =>
+            P8 bop r lr x y lx ly zx zy x0 x1 x2 x3 x4
+        | S_Scope _ _ decls s ev_s ev_s' x x0 => P9 decls s ev_s ev_s' x x0
+        end *)
+
+
+
+    End Induction.
+
+    Definition gmp_stmt_sem := @generic_stmt_sem _gmp_statement _gmp_t _gmp_stmt_sem _gmp_stmt_vars.
+
+    Definition gmp_pgrm_sem := 
+        @generic_pgrm_sem Empty_set _gmp_statement _gmp_t _gmp_stmt_sem _gmp_stmt_vars (fun _ => T_Ext Mpz)  build_rac_fenv.
+
+End GMPSemantics.
+
 Notation "ev |= s => ev'" := (fun f => gmp_stmt_sem f ev s ev') : gmp_stmt_sem_scope.
 
-Definition gmp_pgrm_sem := 
-    @generic_pgrm_sem Empty_set _gmp_statement _gmp_t (fun _ => T_Ext Mpz) Empty_exp_sem _gmp_stmt_sem _gmp_stmt_vars build_rac_fenv.
+
+#[global] Hint Constructors _gmp_stmt_sem  : rac_hint.
