Arithmetic/theories/Languages/MiniC/Lemmas.v
@@ -8,332 +8,361 @@ Import FunctionalEnv Domain.
 #[local] Open Scope utils_scope.
 
 
-Lemma LC1_weakening_of_expression_semantics {T} : 
-    forall exp_sem, 
-    (_LC1_weakening_of_expression_semantics exp_sem exist_env_mem_partial_order)
-    ->
-    _LC1_weakening_of_expression_semantics (@generic_exp_sem T exp_sem) exist_env_mem_partial_order
-.
-Proof with (eauto using refl_env_mem_partial_order with rac_hint).
-    split...  intro Hderiv. induction Hderiv; intros...
-        constructor. eapply eq_int_env_mem_partial_order...
-Qed.
+Section GenericLemmas.
+    Context {S T : Set} {ext_stmt_vars : S -> StringSet.t} {fe : @fenv S T}.
+    
+    Variable (exp_sem : forall e, @generic_exp_sem_sig T e).
+    Variable (stmt_sem : forall f e, @generic_stmt_sem_sig S T f e).
 
+    Variable (_determinist_stmt_eval :  _determinist_stmt_eval generic_exp_sem stmt_sem (fe := fe)).
 
-Definition weakening_of_c_expression_semantics {T} := LC1_weakening_of_expression_semantics (@Empty_exp_sem T) weakening_of_empty_expression_semantics. 
+    Notation generic_exp_sem := (fun e => @generic_exp_sem T e).
+    Notation generic_stmt_sem := (fun f e => @generic_stmt_sem _ _ stmt_sem ext_stmt_vars f e).
 
 
 
-Lemma LC21_weakening_of_expression_semantics {S T : Set} : 
-    forall exp_sem stmt_sem ext_stmt_vars, 
-    _LC21_weakening_of_expression_semantics exp_sem stmt_sem env_mem_partial_order
-    -> _LC21_weakening_of_expression_semantics exp_sem (@generic_stmt_sem S T exp_sem stmt_sem ext_stmt_vars) env_mem_partial_order
-.
-Proof with eauto using refl_env_mem_partial_order, env_partial_order_add with rac_hint.
-    intros exp_sem stmt_sem ext_stmt_vars Hext_stmt Hext_exp f ev₀ s ev₁. 
-    pose proof (LC1_weakening_of_expression_semantics exp_sem Hext_exp) as exp_weak.
-    intro Hderiv. induction Hderiv ; intros ev₀' sub Henvmem.
+    Lemma LC1_weakening_of_expression_semantics : 
+        _LC1_weakening_of_expression_semantics exp_sem exist_env_mem_partial_order ->
+        _LC1_weakening_of_expression_semantics generic_exp_sem exist_env_mem_partial_order
+    .
+    Proof with (eauto using refl_env_mem_partial_order with rac_hint).
+        split...  intro Hderiv. induction Hderiv; intros...
+            constructor. eapply eq_int_env_mem_partial_order...
+    Qed.
+
+
+    Lemma LC21_weakening_of_statement_semantics : 
+        _LC21_weakening_of_statement_semantics generic_exp_sem stmt_sem exist_env_mem_partial_order env_mem_partial_order (fe:=fe) ->
+        _LC21_weakening_of_statement_semantics  generic_exp_sem generic_stmt_sem exist_env_mem_partial_order env_mem_partial_order (fe:=fe)
+    .
+    Proof with eauto using refl_env_mem_partial_order, env_partial_order_add with rac_hint.
+        intros  Hext_stmt exp_weak ev₀ s ev₁. red in exp_weak.
+
+        intro Hderiv.  induction Hderiv using @generic_stmt_sem_full_ind ; intros ev₀' sub Henvmem.
+
         (* skip *)
-        * exists ev₀'. split...
+        - exists ev₀'. split...
         
         (* assign *) 
-        * exists (ev₀' <| env ; vars ::= {{x \induced (proj1_sig sub) z}} |>). split. 
+        - exists (ev₀' <| env ; vars ::= {{x \induced (proj1_sig sub) z}} |>). split. 
             + simpl. pose proof (env_partial_order_add ev ev₀' sub) as H3. simpl in *. now  destruct H3 with x z.
             + apply S_Assign...
-                ** apply env_same_ty with ev...
-                    *** right. now exists sub.
-                     *** congruence.
-                ** rewrite (exp_weak e) in H1. specialize (H1 ev₀'). destruct H1... now exists sub.
+                -- apply env_same_ty with ev...
+                    ++ right. now exists sub.
+                    ++ congruence.
+                -- rewrite exp_weak in H1. specialize (H1 ev₀'). destruct H1... now exists sub.
 
         (* if true *)
-        * destruct H. destruct (IHHderiv ev₀' sub) as [ev_s [Henvmem2 Hderiv2]]...
+        - destruct H as [H1 H2]. destruct (IHHderiv ev₀' sub) as [ev_s [Henvmem2 Hderiv2]]...
             exists ev_s. split...
             apply S_IfTrue with z... split... 
-            rewrite  (exp_weak e) in H. apply H. now exists sub.
+            rewrite  exp_weak in H1. apply H1. now exists sub.
 
         (* if false *)
-        * destruct (IHHderiv ev₀' sub) as [ev_s [Henvmem2 Hderiv2]]... exists ev_s. split...
+        - destruct (IHHderiv ev₀' sub) as [ev_s [Henvmem2 Hderiv2]]... exists ev_s. split...
             apply S_IfFalse...
-            rewrite  (exp_weak e) in H. apply H. now exists sub. 
+            rewrite exp_weak in H. apply H. now exists sub. 
 
 
-         (* while *)
-        * destruct (IHHderiv ev₀' sub) as [ev_s [Henvmem2 Hderiv2]]...
+        (* while *)
+        - destruct (IHHderiv ev₀' sub) as [ev_s [Henvmem2 Hderiv2]]...
 
 
         (* c seq *)
-        * destruct (IHHderiv ev₀' sub) as [I1ev [I1Hrel I1Hderiv]]... 
-            destruct (IHHderiv0 I1ev sub) as [I2ev [I2Hrel I2Hderiv]]... 
+        - destruct (IHHderiv1 ev₀' sub) as [I1ev [I1Hrel I1Hderiv]]... 
+            destruct (IHHderiv2 I1ev sub) as [I2ev [I2Hrel I2Hderiv]]... 
 
         (* f call *)
-         * destruct (IHHderiv (empty_env <| env; vars ::= p_map_addall_back xargs vargs |>) sub) as [b_ev' [H5 Hsem]]; subst vargs.
+        
+        - destruct (IHHderiv (empty_env <| env; vars ::= p_map_addall_back xargs vargs |>) sub) as [b_ev' [Henvmem2 Hsem2]]; subst vargs.
             +  apply same_int_any_sub. 
-                ++ apply List.Forall2_length in H1. pose proof (List.map_length  (fun x : Int.MI => Def (VInt x)) zargs) as H5.
-                    rewrite H5 in H1. congruence. 
-                ++ apply empty_env_mem_refl_any_sub. 
+                * apply List.Forall2_length in H1. pose proof (List.map_length  (fun x : Int.MI => Def (VInt x)) zargs) as Hlength.
+                    rewrite Hlength in H1. congruence. 
+                * apply empty_env_mem_refl_any_sub. 
             + eexists (ev₀' <| env; vars ::= {{c \Def z}} |> <| mstate := b_ev' |>). split.
-                ++ apply env_mem_partial_order_add_mem... now pose proof (env_partial_order_add ev ev₀' _ Henvmem c z).
-                ++  apply S_FCall with b xargs zargs...
-                    +++ epose proof (List.Forall2_impl (R1:=generic_exp_sem ev) (generic_exp_sem ev₀')) as Hforall.
+                * apply env_mem_partial_order_add_mem... now pose proof (env_partial_order_add ev ev₀' _ Henvmem c z).
+                *  apply S_FCall with b xargs zargs...
+                    -- epose proof (List.Forall2_impl (R1:=generic_exp_sem ev) (generic_exp_sem ev₀')) as Hforall. red. repeat split...
                             apply Hforall... intros. apply exp_weak with ev... now exists sub.
-                    +++ apply eq_int_env_mem_partial_order with b_ev... now exists sub. 
-
+                    -- apply eq_int_env_mem_partial_order with b_ev... now exists sub. 
+        
         (* p call *)
-         * destruct (IHHderiv (empty_env <| env; vars ::= p_map_addall_back xargs vargs |>) sub) as [b_ev' [H5 Hsem]]; subst vargs.
+        - destruct (IHHderiv (empty_env <| env; vars ::= p_map_addall_back xargs vargs |>) sub) as [b_ev' [H5 Hsem2]]; subst vargs.
             +  apply same_int_any_sub. 
-                ++ apply List.Forall2_length in H1. pose proof (List.map_length  (fun x : Int.MI => Def (VInt x)) zargs) as H5.
+                * apply List.Forall2_length in H1. pose proof (List.map_length  (fun x : Int.MI => Def (VInt x)) zargs) as H5.
                     rewrite H5 in H1. congruence. 
-                ++ apply empty_env_mem_refl_any_sub. 
+                * apply empty_env_mem_refl_any_sub. 
             + exists (ev₀' <| mstate := b_ev' |>). split.
-                ++ apply env_mem_partial_order_add_mem...
-                ++  apply S_PCall with b xargs zargs...
-                    +++ epose proof (List.Forall2_impl (R1:=generic_exp_sem ev) (generic_exp_sem ev₀')) as Hforall.
-                            apply Hforall... intros. apply exp_weak with ev... now exists sub.
-
+                * apply env_mem_partial_order_add_mem...
+                *  apply S_PCall with b xargs zargs...
+                    epose proof (List.Forall2_impl (R1:=generic_exp_sem ev) (generic_exp_sem ev₀')) as Hforall. red. repeat split...
+                    apply Hforall... intros. apply exp_weak with ev... now exists sub.
+    
         (* return *)
-        * exists (ev₀' <| env ; vars ::= {{res_f \Def z}} |>). split.
+        - exists (ev₀' <| env ; vars ::= {{res_f \Def z}} |>). split.
             + now pose proof (env_partial_order_add ev ev₀' sub Henvmem).
             + apply S_Return... apply (exp_weak e ev z)... now exists sub.
 
         (* assert *)
-        * exists ev₀'. split... apply S_PAssert with z...
+        - exists ev₀'. split... apply S_PAssert with z...
             apply (exp_weak e ev z)... now exists sub.
 
         (* other cases *)
-        * specialize (Hext_stmt Hext_exp f ev (S_Ext s) ev').
-            eapply Hext_stmt in H... destruct H as [ev'' [Hrel2 Hderiv]]...                  
-Qed.
+        - specialize (Hext_stmt exp_weak ev (S_Ext s) ev').
+            eapply Hext_stmt in H... destruct H as [ev'' [Hrel2 Hderiv2]]...                  
+    Qed.
 
-Definition weakening_of_c_statements_semantics_1 {S T} := 
-    LC21_weakening_of_expression_semantics (@Empty_exp_sem T) (@Empty_stmt_sem S T) Empty_ext_stmt_vars (weakening_of_empty_statement_semantics_1 env_mem_partial_order).  
+    Lemma LC22_weakening_of_statement_semantics : 
+        _LC22_weakening_of_statement_semantics exp_sem stmt_sem exist_env_mem_partial_order env_mem_partial_order (fe:=fe) -> 
+        _LC22_weakening_of_statement_semantics exp_sem generic_stmt_sem exist_env_mem_partial_order env_mem_partial_order (fe:=fe)
+    .
+    Proof with auto with rac_hint.
+        intros Hext_stmt Hext_exp  ev₀ ev₀' s ev₁ sub [Hderiv1 Hrel]. 
+        pose proof (LC1_weakening_of_expression_semantics Hext_exp ) as exp_weak.
+        generalize dependent ev₀'. generalize dependent sub.
+        induction Hderiv1 using @generic_stmt_sem_full_ind; intros sub ev₀' Hrel ev₁' Hderiv2 ; inversion Hderiv2 ; subst ; try easy...
 
-Lemma LC22_weakening_of_expression_semantics {S T : Set} : 
-    forall exp_sem stmt_sem ext_stmt_vars, 
-    _LC22_weakening_of_expression_semantics exp_sem stmt_sem env_mem_partial_order
-    -> _LC22_weakening_of_expression_semantics exp_sem (@generic_stmt_sem S T exp_sem stmt_sem ext_stmt_vars) env_mem_partial_order
-.
-Proof with auto with rac_hint.
-    intros  exp_sem stmt_sem ext_stmt_vars Hext_stmt Hdeter Hext_exp  f ev₀ ev₀' s ev₁ sub [Hderiv1 Hrel]. 
-    pose proof (LC1_weakening_of_expression_semantics exp_sem Hext_exp) as exp_weak.
-    unfold _LC22_weakening_of_expression_semantics in Hext_stmt. 
-    unfold _LC1_weakening_of_expression_semantics in Hext_exp.    
-    generalize dependent ev₀'. generalize dependent sub.
-    induction Hderiv1 ; intros sub ev₀' Hrel ev₁' Hderiv2 ; inversion Hderiv2 ; subst ; try easy...
+        (* assign *)
+        - split... simpl. intros v [Hnotin Hnotcompvar].  assert (HH: type_of_value (ev x) <> None) by congruence. apply type_of_value_env in HH.
+            apply not_in_diff with (x:=v)  in HH...
+            autounfold with rac_hint. eapply p_map_not_same_eq...  intro neq...
 
-    (* assign *)
-    - split... simpl. intros v [Hnotin Hnotcompvar].  assert (HH: type_of_value (ev x) <> None) by congruence. apply type_of_value_env in HH.
-        apply not_in_diff with (x:=v)  in HH... autounfold with rac_hint. eapply p_map_not_same_eq...  intro neq...
-
-    (* if false *)
-    - apply IHHderiv1... destruct H. specialize (exp_weak e ev z). rewrite exp_weak in H. specialize (H ev₀'). 
-            apply determinist_exp_eval in H...
-                + apply H in H5. inversion H5. now subst.
-                + now exists sub.
-
-    (* if true *)
-    -  destruct H5. specialize (exp_weak e ev (VInt zero)). rewrite exp_weak in H. specialize (H ev₀').
-            apply determinist_exp_eval in H...
-            + apply H in H1. inversion H1. now subst.
+        (* if false && if true  *)
+        - exfalso. destruct H as [H Hnotzero]. red in exp_weak. specialize (exp_weak e ev z). 
+            apply exp_weak with ev₀' in H.
+            + apply determinist_exp_eval in H4. apply H4 in H. inversion H. now apply Hnotzero.  
             + now exists sub.
 
-    (* seq *)
-    - admit. 
-    
-    (* fcall *)
-    - rewrite H9 in H0. inversion H0. subst. clear H0 H9 H8 H14. split ; admit.
+        (* if true && if false  *)
+        - exfalso. destruct H4 as [H8 Hnotzero]. red in exp_weak. specialize (exp_weak e ev zero). 
+            eapply exp_weak in H.
+            + apply determinist_exp_eval in H8. apply H8 in H. inversion H. now apply Hnotzero.  
+            + now exists sub.
+        
+        (* seq *) 
+        - admit.  
+        
+        (* fcall *)
+        - destruct H7 as (Hl & Hf & Hforall & Hsem). rewrite Hf in H0. admit.
+        
+        (* pcall *)
+        - destruct H5 as (Hl & Hf & Hforall & Hsem).  rewrite Hf in H0. injection H0 as H0. subst. 
+            edestruct IHHderiv1...
+            + admit.
+            + admit.
+            + epose proof (List.Forall2_impl (R1:=generic_exp_sem ev) (generic_exp_sem ev)) as Hforall2. admit.
 
-    (* pcall *)
-    - rewrite H6 in H0. injection H0 as H0. subst. edestruct IHHderiv1... admit. admit.
-        epose proof (List.Forall2_impl (R1:=generic_exp_sem ev) (generic_exp_sem ev)) as Hforall. admit.
 
-    (* return *)
-    -  split ; intros v... intros [Hnotin Hnotcomp]. destruct (string_dec res_f v).
-        + subst. discriminate. (* v is the function return value*)
-        +  symmetry. apply p_map_not_same...
+        (* return *)
+        -  split ; intros v... intros [Hnotin Hnotcomp]. destruct (string_dec res_f v).
+            + subst. discriminate. (* v is the function return value*)
+            +  symmetry. apply p_map_not_same...
+                
+
+        (* ext *)
+        - eapply Hext_stmt.
+            +  apply Hext_exp.
+            + split... apply H.
+            + apply H1.
+    Admitted.
+
+
+
+    Fact LC1_weakening_of_expression_semantics_3  : 
+        _LC1_weakening_of_expression_semantics_3 exp_sem strong_env_mem_partial_order ->
+        _LC1_weakening_of_expression_semantics_3 generic_exp_sem strong_env_mem_partial_order
+    .
+    Proof with eauto with rac_hint.
+        intros Hextweak ev e v sub Hderiv.
+        induction Hderiv; intros ev' Henvmem [HnotinEnv HnotinMem].
+        - constructor.
+        - assert (HxnotinEnv: ~ (dom ev - dom ev')%dom_ x). {
+            intros contra.  apply (HnotinEnv x contra); now left.
+            }  
+            apply not_in_sub_domain_prop in HxnotinEnv;[|apply in_domain_dec| apply in_domain_dec].
+            constructor. destruct HxnotinEnv.
+            * destruct H0 as [z' Hevx]. destruct Henvmem as [Henv _]. specialize (Henv x _ _ Hevx). rewrite H in Henv. inversion Henv. 
+                destruct z' eqn:Z'Eqn.
+                + destruct v eqn:VEqn.
+                    ++ simpl in H1. inversion H1. now subst.
+                    ++ destruct l; now subst.
+                + simpl in H1. now subst.
+            * exfalso. apply H0. now exists z. 
+        
+        - apply C_E_BinOpInt with z_ir z'_ir.
+            + apply IHHderiv1...
+                * split.
+                    -- intros v Hdom. apply HnotinEnv in Hdom. simpl in Hdom |- *. StringSet.D.fsetdec. 
+                    -- intros.  apply HnotinMem in H0. destruct H0 as [x0 [Hevx0 HnotInx0]].
+                        exists x0. split... simpl in HnotInx0. StringSet.D.fsetdec.
+            + apply IHHderiv2...
+                * split.
+                    -- intros v Hdom. apply HnotinEnv in Hdom. simpl in Hdom |- *. 
+                        StringSet.D.fsetdec.
+                    -- intros.  apply HnotinMem in H0. destruct H0 as [x0 [Hevx0 HnotInx0]].
+                        exists x0. split... simpl in HnotInx0. StringSet.D.fsetdec.
+
+        - eapply C_E_BinOpTrue...
+            + apply IHHderiv1...
+                * split.
+                    -- intros v Hdom. apply HnotinEnv in Hdom. simpl in Hdom |- *. StringSet.D.fsetdec.
+                    -- intros.  apply HnotinMem in H0. destruct H0 as [x0 [Hevx0 HnotInx0]].
+                        exists x0. split... simpl in HnotInx0. StringSet.D.fsetdec.
+            + apply IHHderiv2...
+                * split.
+                    -- intros v Hdom. apply HnotinEnv in Hdom. simpl in Hdom |- *. StringSet.D.fsetdec.
+                    -- intros. apply HnotinMem in H0. destruct H0 as [x0 [Hevx0 HnotInx0]].
+                        exists x0. split... simpl in HnotInx0. StringSet.D.fsetdec.
+
+        - eapply C_E_BinOpFalse...
+            + apply IHHderiv1...
+                * split.
+                    -- intros v Hdom. apply HnotinEnv in Hdom. simpl in Hdom |- *. StringSet.D.fsetdec.
+                    -- intros.  apply HnotinMem in H0. destruct H0 as [x0 [Hevx0 HnotInx0]].
+                        exists x0. split... simpl in HnotInx0. StringSet.D.fsetdec.
+            + apply IHHderiv2...
+                * split.
+                    -- intros v Hdom. apply HnotinEnv in Hdom. simpl in Hdom |- *. StringSet.D.fsetdec.
+                    -- intros.  apply HnotinMem in H0. destruct H0 as [x0 [Hevx0 HnotInx0]].
+                        exists x0. split... simpl in HnotInx0. StringSet.D.fsetdec.
+    Qed.
+
+
+
+    Lemma LC23_weakening_of_statement_semantics : 
+        _LC1_weakening_of_expression_semantics_3 exp_sem strong_env_mem_partial_order -> 
+        _LC23_weakening_of_statement_semantics stmt_sem strong_env_mem_partial_order (ext_stmt_vars:=ext_stmt_vars) (fe:=fe) -> 
+        _LC23_weakening_of_statement_semantics generic_stmt_sem strong_env_mem_partial_order  (ext_stmt_vars:=ext_stmt_vars) (fe:=fe)
+    .
+    Proof with eauto with rac_hint; try easy.
+        intros ext_exp_weak ext_stmt_weak.
+        epose proof (LC1_weakening_of_expression_semantics_3 ext_exp_weak) as exp_weak.
+        epose proof (determinist_stmt_eval _ _determinist_stmt_eval) as stmt_deter.
+        intros ev₀ s ev₁ sub Hderiv.
+        induction Hderiv using @generic_stmt_sem_full_ind; intros ev₀' Hrel [Henv Hmem]. 
+        
+        (* skip *)
+        - exists ev₀'. constructor.
+
+        (* assign *)
+        - exists (ev₀' <| env ; vars ::= {{x\Def z}} |>). apply S_Assign...
+            + apply env_same_ty with ev... left. pose proof strong_env_mem_stronger. exists sub. now apply strong_env_mem_stronger. 
+            + eapply LC1_weakening_of_expression_semantics_3... split. 
+                * intros v Hdom. apply Henv in Hdom. simpl in Hdom |- *. StringSet.D.fsetdec.
+                * intros l Hdom. apply Hmem in Hdom as [l' Hdom]. simpl in Hdom |- *. exists l'. destruct Hdom.  split...
+                    StringSet.D.fsetdec. 
+
+        (* if true *)
+        - edestruct IHHderiv... 
+            + split. 
+                * intros v Hdom. specialize (Henv v Hdom). simpl in Henv. StringSet.D.fsetdec.
+                * intros l Hdom. apply Hmem in Hdom as [l' Hdom]. simpl in Hdom |- *. exists l'. destruct Hdom.  split...
+                    StringSet.D.fsetdec. 
+            + exists x. apply S_IfTrue with z...
+                split... eapply LC1_weakening_of_expression_semantics_3... split.
+                * intros v Hdom. apply Henv in Hdom. simpl in Hdom |- *. StringSet.D.fsetdec.
+                * intros l Hdom. apply Hmem in Hdom as [l' Hdom]. simpl in Hdom |- *. exists l'. destruct Hdom.  split...
+                    StringSet.D.fsetdec. 
+
+
+        (* if false *)
+        - edestruct IHHderiv... 
+            + split. 
+                * intros v Hdom. apply Henv in Hdom. simpl in Hdom |- *. StringSet.D.fsetdec.
+                * intros l Hdom. apply Hmem in Hdom as [l' Hdom]. simpl in Hdom |- *. exists l'. destruct Hdom.  split...
+                    StringSet.D.fsetdec. 
+            + exists x. apply S_IfFalse...
+                eapply LC1_weakening_of_expression_semantics_3... split.
+                * intros v Hdom. apply Henv in Hdom. simpl in Hdom |- *. StringSet.D.fsetdec.
+                * intros l Hdom. apply Hmem in Hdom as [l' Hdom]. simpl in Hdom |- *. exists l'. destruct Hdom.  split...
+                    StringSet.D.fsetdec. 
+
+        (* while *)
+        - edestruct IHHderiv... split.
+            + intros v Hdom. apply Henv in Hdom. simpl in Hdom |- *. StringSet.D.fsetdec.
+            + intros l Hdom. apply Hmem in Hdom as [l' Hdom]. simpl in Hdom |- *. exists l'. destruct Hdom.  split...
+                StringSet.D.fsetdec. 
             
-    (* assert *)
-    - eapply Hext_stmt with (ev₀:=ev) (ev₁:=ev')  in H1...
-Admitted.
+
+        (* seq *)
+        - admit. 
+
+        (* fcall *)
+        - destruct IHHderiv with ((empty_env <| env; vars ::= p_map_addall_back xargs vargs |>))...
+            + admit. (* need refl env *)
+            + split.
+                * intros. exfalso.  apply (d_sub_d_empty (empty_env <| env; vars ::= p_map_addall_back xargs vargs |>)).
+                    now exists v.
+                * intros. exfalso.  apply (d_sub_d_empty (empty_env <| env; vars ::= p_map_addall_back xargs vargs |>).(mstate)). 
+                    now exists x.
+            + clear IHHderiv. exists (ev₀' <| env ; vars ::= {{c\Def z}} |> <| mstate := x |>). econstructor...
+                * repeat split...
+                    eapply (List.Forall2_impl (R1:=generic_exp_sem ev) (generic_exp_sem ev₀'))...
+                    intros. eapply LC1_weakening_of_expression_semantics_3... split.
+                    -- intros v Hdom. apply Henv in Hdom. simpl in Hdom |- *. StringSet.D.fsetdec || admit.
+                    -- intros l Hdom. apply Hmem in Hdom as [l' Hdom]. simpl in Hdom |- *. exists l'. destruct Hdom.  split...
+                        StringSet.D.fsetdec || admit.
 
 
-Definition weakening_of_c_statements_semantics_2 {S T} := 
-    LC22_weakening_of_expression_semantics (@Empty_exp_sem T) (@Empty_stmt_sem S T) Empty_ext_stmt_vars 
-    (weakening_of_empty_statement_semantics_2 env_mem_partial_order). 
+                * apply stmt_deter in Hderiv...
+                    -- apply Hderiv in H4. now subst. 
+                    -- apply determinist_exp_eval.
+        (* pcall *)
+        - destruct IHHderiv with ((empty_env <| env; vars ::= p_map_addall_back xargs vargs |>))...
+            + admit. (* need refl env *)
+            + split.
+                * intros. exfalso.  apply (d_sub_d_empty (empty_env <| env; vars ::= p_map_addall_back xargs vargs |>)).
+                    now exists v.
+                * intros. exfalso.  apply (d_sub_d_empty (empty_env <| env; vars ::= p_map_addall_back xargs vargs |>).(mstate)). 
+                    now exists x.
+            + clear IHHderiv. exists (ev₀' <| mstate := x |>). econstructor...  repeat split...
+                eapply (List.Forall2_impl (R1:=generic_exp_sem ev) (generic_exp_sem ev₀'))...
+                intros. eapply LC1_weakening_of_expression_semantics_3... split.
+                * intros v Hdom. apply Henv in Hdom. simpl in Hdom |- *. StringSet.D.fsetdec || admit.
+                * intros l Hdom. apply Hmem in Hdom as [l' Hdom]. simpl in Hdom |- *. exists l'. destruct Hdom.  split...
+                    StringSet.D.fsetdec || admit.
+
+        (* return *)
+        - exists (ev₀' <| env ; vars ::= {{res_f\Def z}} |>). apply S_Return.
+            eapply LC1_weakening_of_expression_semantics_3 in H...
+            
+        (* assert *)
+        - exists ev₀'. apply S_PAssert with z...         
+
+        (* other cases *)
+        - unfold _LC23_weakening_of_statement_semantics in ext_stmt_weak.
+            edestruct ext_stmt_weak...
+    Admitted.
+End GenericLemmas.
 
 
-Fact LC1_weakening_of_expression_semantics_3 {T : Set} : forall exp_sem, 
-    _LC1_weakening_of_expression_semantics_3 exp_sem strong_env_mem_partial_order
-    -> _LC1_weakening_of_expression_semantics_3 (@generic_exp_sem T exp_sem) strong_env_mem_partial_order
-.
-Proof with eauto with rac_hint.
-    intros exp Hextweak ev e v sub Hderiv.
-    induction Hderiv; intros ev' Henvmem [HnotinEnv HnotinMem].
-    - constructor.
-    - assert (HxnotinEnv: ~ (dom ev - dom ev')%dom_ x). {
-        intros contra.  apply (HnotinEnv x contra); now left.
-        }  
-        apply not_in_sub_domain_prop in HxnotinEnv;[|apply in_domain_dec| apply in_domain_dec].
-        constructor. destruct HxnotinEnv.
-        * destruct H0 as [z' Hevx]. destruct Henvmem as [Henv _]. specialize (Henv x _ _ Hevx). rewrite H in Henv. inversion Henv. 
-            destruct z' eqn:Z'Eqn.
-            + destruct v eqn:VEqn.
-                ++ simpl in H1. inversion H1. now subst.
-                ++ destruct l; now subst.
-            + simpl in H1. now subst.
-        * exfalso. apply H0. now exists z. 
-    
-    - apply C_E_BinOpInt with z_ir z'_ir.
-        + apply IHHderiv1...
-            * split.
-                ** intros v Hdom. apply HnotinEnv in Hdom. simpl in Hdom. StringSet.D.fsetdec. 
-                ** intros.  apply HnotinMem in H0. destruct H0 as [x0 [Hevx0 HnotInx0]].
-                    exists x0. split... simpl in HnotInx0. StringSet.D.fsetdec.
-        + apply IHHderiv2...
-            * split.
-                ** intros v Hdom. apply HnotinEnv in Hdom. simpl in Hdom. 
-                    StringSet.D.fsetdec.
-                ** intros.  apply HnotinMem in H0. destruct H0 as [x0 [Hevx0 HnotInx0]].
-                    exists x0. split... simpl in HnotInx0. StringSet.D.fsetdec.
 
-    - eapply C_E_BinOpTrue...
-        + apply IHHderiv1...
-            * split.
-                ** intros v Hdom. apply HnotinEnv in Hdom. simpl in Hdom. StringSet.D.fsetdec.
-                ** intros.  apply HnotinMem in H0. destruct H0 as [x0 [Hevx0 HnotInx0]].
-                    exists x0. split... simpl in HnotInx0. StringSet.D.fsetdec.
-        + apply IHHderiv2...
-            * split.
-                ** intros v Hdom. apply HnotinEnv in Hdom. simpl in Hdom. StringSet.D.fsetdec.
-                ** intros. apply HnotinMem in H0. destruct H0 as [x0 [Hevx0 HnotInx0]].
-                    exists x0. split... simpl in HnotInx0. StringSet.D.fsetdec.
+Definition weakening_of_c_expression_semantics {T} := 
+    LC1_weakening_of_expression_semantics 
+        (@Empty_exp_sem T) 
+        weakening_of_empty_expression_semantics. 
 
-    - eapply C_E_BinOpFalse...
-        + apply IHHderiv1...
-            * split.
-                ** intros v Hdom. apply HnotinEnv in Hdom. simpl in Hdom. StringSet.D.fsetdec.
-                ** intros.  apply HnotinMem in H0. destruct H0 as [x0 [Hevx0 HnotInx0]].
-                    exists x0. split... simpl in HnotInx0. StringSet.D.fsetdec.
-        + apply IHHderiv2...
-            * split.
-                ** intros v Hdom. apply HnotinEnv in Hdom. simpl in Hdom. StringSet.D.fsetdec.
-                ** intros.  apply HnotinMem in H0. destruct H0 as [x0 [Hevx0 HnotInx0]].
-                    exists x0. split... simpl in HnotInx0. StringSet.D.fsetdec.
-Qed.
 
 Definition weakening_of_c_expression_semantics_3 {T} := 
-    LC1_weakening_of_expression_semantics_3 (@Empty_exp_sem T) (weakening_of_empty_expression_semantics_3 strong_env_mem_partial_order). 
+    @LC1_weakening_of_expression_semantics_3  T
+        (@Empty_exp_sem T) 
+        (weakening_of_empty_expression_semantics_3 strong_env_mem_partial_order). 
 
 
-Lemma LC23_weakening_of_expression_semantics {S T : Set} : 
-    forall exp_sem stmt_sem ext_stmt_vars, 
-    _LC1_weakening_of_expression_semantics_3 exp_sem strong_env_mem_partial_order
-    -> _LC23_weakening_of_expression_semantics stmt_sem ext_stmt_vars  strong_env_mem_partial_order
-    -> _LC23_weakening_of_expression_semantics (@generic_stmt_sem S T exp_sem stmt_sem ext_stmt_vars) ext_stmt_vars strong_env_mem_partial_order
-.
-
-Proof with eauto with rac_hint; try easy.
-    intros exp_sem stmt_sem ext_stmt_vars ext_exp_weak ext_stmt_weak.
-    epose proof (LC1_weakening_of_expression_semantics_3 exp_sem ext_exp_weak) as exp_weak.
-    intros f ev₀ s ev₁ sub Hderiv. 
-
-    induction Hderiv; intros ev₀' Hrel [Henv Hmem]. 
-    (* skip *)
-    - exists ev₀'. constructor.
-
-    (* assign *)
-    -  exists (ev₀' <| env ; vars ::= {{x\Def z}} |>). apply S_Assign...
-        +  apply env_same_ty with ev... left. pose proof strong_env_mem_stronger. exists sub. now apply H2. 
-        + eapply LC1_weakening_of_expression_semantics_3... split. 
-            * intros v Hdom. apply Henv in Hdom. simpl in Hdom. StringSet.D.fsetdec.
-            * intros l Hdom. apply Hmem in Hdom as [l' Hdom]. simpl in Hdom. exists l'. destruct Hdom.  split...
-                StringSet.D.fsetdec. 
-
-    (* if true *)
-    - destruct H as [He Hnotzero]. edestruct IHHderiv... 
-        * split. 
-            + intros v H. specialize (Henv v H). simpl in Henv. StringSet.D.fsetdec.
-            + intros x H. specialize (Hmem x H). simpl in Hmem.
-            destruct Hmem as [v [Hmpz Hmem]]. exists v. split... StringSet.D.fsetdec.
-        * exists x. apply S_IfTrue with z...
-            split... eapply LC1_weakening_of_expression_semantics_3... split.
-            + intros v Hdom. apply Henv in Hdom. simpl in Hdom. StringSet.D.fsetdec.
-            + intros l Hdom. apply Hmem in Hdom as [l' Hdom]. simpl in Hdom.  exists l'. destruct Hdom. split...
-                StringSet.D.fsetdec.
+Definition weakening_of_c_statements_semantics_1 {S T}  f := 
+    @LC21_weakening_of_statement_semantics S T Empty_ext_stmt_vars f
+    (@Empty_stmt_sem S T) 
+    (weakening_of_empty_statement_semantics_1 exist_env_mem_partial_order env_mem_partial_order f  generic_exp_sem).  
 
 
-    (* if false *)
-    - edestruct IHHderiv... 
-        * split. 
-            + intros v Hdom. specialize (Henv v Hdom). simpl in Henv. StringSet.D.fsetdec.
-            + intros x Hdom. specialize (Hmem x Hdom). simpl in Hmem.
-            destruct Hmem as [v [Hmpz Hmem]]. exists v. split... StringSet.D.fsetdec.
-
-        * exists x. apply S_IfFalse... eapply LC1_weakening_of_expression_semantics_3... split.
-            + intros v Hdom. apply Henv in Hdom. simpl in Hdom. StringSet.D.fsetdec. 
-            + intros l Hdom. apply Hmem in Hdom as [l' Hdom]. simpl in Hdom.  exists l'. destruct Hdom. split...
-                StringSet.D.fsetdec.
+Definition weakening_of_c_statements_semantics_2 {S T} f := 
+    @LC22_weakening_of_statement_semantics S T Empty_ext_stmt_vars f (@Empty_exp_sem T) (@Empty_stmt_sem S T) 
+    (weakening_of_empty_statement_semantics_2 exist_env_mem_partial_order env_mem_partial_order f (@Empty_exp_sem T)). 
 
 
-    (* while *)
-    - edestruct IHHderiv... split.
-        *  intros v Hdom. specialize (Henv v Hdom). simpl in *. StringSet.D.fsetdec.
-        * intros x Hdom. specialize (Hmem x Hdom). simpl in Hmem.
-            destruct Hmem as [v [Hmpz Hmem]]. exists v. split...  simpl. StringSet.D.fsetdec.
-        
 
-    (* seq *)
-    - admit. 
-
-    (* fcall *)
-    - destruct IHHderiv with ((empty_env <| env; vars ::= p_map_addall_back xargs vargs |>))...
-        * admit. (* need refl env *)
-        * split.
-            + intros. exfalso.  apply (d_sub_d_empty (empty_env <| env; vars ::= p_map_addall_back xargs vargs |>)).
-                now exists v.
-            + intros. exfalso.  apply (d_sub_d_empty (empty_env <| env; vars ::= p_map_addall_back xargs vargs |>).(mstate)). 
-                now exists x.
-        * clear IHHderiv. exists (ev₀' <| env ; vars ::= {{c\Def z}} |> <| mstate := x |>). econstructor...
-            + eapply (List.Forall2_impl (R1:=generic_exp_sem ev) (generic_exp_sem ev₀'))...
-                intros. assert (List.In a eargs) by admit. 
-                eapply LC1_weakening_of_expression_semantics_3... split.
-                ++ intros. apply Henv in H8. intros contra. apply H8. simpl. admit.
-                ++ intros. apply Hmem in H8. destruct H8 as [v [Hev Hnotin]]. exists v. split... 
-                    intros contra. apply Hnotin. simpl. admit.
-            + assert (_determinist_exp_eval exp_sem) by admit. 
-            assert (_determinist_stmt_eval exp_sem stmt_sem) by admit. 
-                pose proof (determinist_stmt_eval _ _ _ H7 H6 _ _ _ _ H2 _ H5). now subst. 
-    
-    (* pcall *)
-    - destruct IHHderiv with ((empty_env <| env; vars ::= p_map_addall_back xargs vargs |>))...
-        * admit. (* need refl env *)
-        * split.
-            + intros. exfalso.  apply (d_sub_d_empty (empty_env <| env; vars ::= p_map_addall_back xargs vargs |>)).
-                now exists v.
-            + intros. exfalso.  apply (d_sub_d_empty (empty_env <| env; vars ::= p_map_addall_back xargs vargs |>).(mstate)). 
-                now exists x.
-        * clear IHHderiv. exists (ev₀' <| mstate := x |>). econstructor...
-            + eapply (List.Forall2_impl (R1:=generic_exp_sem ev) (generic_exp_sem ev₀'))...
-                intros. assert (List.In a eargs) by admit. 
-                eapply LC1_weakening_of_expression_semantics_3... split.
-                ++ intros. apply Henv in H6. intros contra. apply H6. simpl. admit.
-                ++ intros. apply Hmem in H6. destruct H6 as [v [Hev Hnotin]]. exists v. split... 
-                    intros contra. apply Hnotin. simpl. admit.
-
-    (* return *)
-    - exists (ev₀' <| env ; vars ::= {{res_f\Def z}} |>). apply S_Return.
-        eapply LC1_weakening_of_expression_semantics_3 in H...
-        
-    (* assert *)
-    - exists ev₀'. apply S_PAssert with z...         
-
-    (* other cases *)
-    - unfold _LC23_weakening_of_expression_semantics in ext_stmt_weak.
-        specialize (ext_stmt_weak f  ev (S_Ext s) _  sub H ev₀' Hrel).
-        destruct ext_stmt_weak as [ev'' Hd]... 
-Admitted.
-
-Definition weakening_of_c_statements_semantics_3 {S T}  := 
-    LC23_weakening_of_expression_semantics 
-    (@Empty_exp_sem T) (@Empty_stmt_sem S T) Empty_ext_stmt_vars 
-    (weakening_of_empty_expression_semantics_3 strong_env_mem_partial_order) 
-    (weakening_of_empty_statement_semantics_3 Empty_ext_stmt_vars strong_env_mem_partial_order). 
+Definition weakening_of_c_statements_semantics_3 {S T} f := 
+    LC23_weakening_of_statement_semantics 
+        (@Empty_exp_sem T) (@Empty_stmt_sem S T) 
+        (weakening_of_empty_expression_semantics_3 strong_env_mem_partial_order) 
+        (weakening_of_empty_statement_semantics_3 strong_env_mem_partial_order Empty_ext_stmt_vars f). 
