Arithmetic/theories/Languages/MiniGMP/Facts.v
@@ -7,60 +7,65 @@ Open Scope Z.
 Import Environnement.Facts.
 Import FunctionalEnv.
 
-Fact _no_mem_aliasing_gmp : _no_mem_aliasing _gmp_stmt_sem.
-Proof with auto with rac_hint.
-    intros exp_sem f ev s ev' Hnoalias H. induction H
-    ; auto ;  try (rename v into l1) ;
-    intros v v' ll l' Hvv' Hl Hl' leq ; subst ; autounfold with rac_hint in * ; simpl in *.
-    - destruct (eq_dec x v).
-        + subst. autounfold with rac_hint in *. rewrite p_map_same in Hl. rewrite p_map_not_same in Hl'... inversion Hl. 
-            subst. now destruct H with v'.
-        + rewrite p_map_not_same in Hl... destruct (eq_dec x v').
-            * subst. rewrite p_map_same in Hl'. inversion Hl'. subst. now destruct H with v.
-            * rewrite p_map_not_same in Hl'... destruct Hnoalias with v v' l' l'...
-    - destruct (eq_dec x v).
-        + subst. now rewrite p_map_same in Hl.
-        + rewrite p_map_not_same in Hl... destruct (eq_dec l' a).
-            * destruct Hnoalias with v x l' a... 
-            * destruct (eq_dec x v').
-                ** subst. rewrite p_map_same in Hl'... easy.
-                ** rewrite p_map_not_same in Hl'... destruct Hnoalias with v v' l' l'...     
-    - destruct (string_dec x v').
-        + subst. rewrite p_map_same in Hl'. discriminate.
-        + rewrite p_map_not_same in Hl'... destruct (string_dec x v).
-            * subst. rewrite p_map_same in Hl... discriminate.
-            * rewrite p_map_not_same in Hl... destruct Hnoalias with v v' l' l'...
-    - assert (type_of_value (Some b) = Some C_Int). {
-        destruct H3 as [sup [inf eq]]. destruct (Z.lt_trichotomy zx zy) as [Hinf | [Heq | Hsup]].
-        - apply inf in Hinf. now subst.
-        - apply eq in Heq. now subst.
-        - apply Z.lt_gt in Hsup.  apply sup in Hsup. now subst. 
-        } 
-        destruct (string_dec c v').
-        + subst. rewrite p_map_same in Hl'. injection Hl' as Hl'. now subst. 
-        + rewrite p_map_not_same in Hl'... destruct (string_dec c v).
-            * subst. rewrite p_map_same in Hl. injection Hl as Hl. now subst.
-            * rewrite p_map_not_same in Hl... destruct Hnoalias with v v' l' l'...
-Qed.
+Section GMPFacts.
 
-(* helper lemma for gmp cmp semantics *)
-Fact cmp_induced : forall zx zy (b: 𝕍) sub,
-    (zx > zy <-> b = one) /\ (zx < zy <-> b = sub_one) /\ (Z.eq zx zy <-> b = zero)
-    -> 
-    (zx > zy <-> induced sub b = one) /\
-(zx < zy <-> induced sub b = sub_one) /\ (Z.eq zx zy <-> induced sub b = zero).
-Proof.
-    intros zx zy b sub (Hone & Hsubone &Hzero). split.
-    - split.
-        * intros Hzxzy. apply Hone in Hzxzy. now subst.
-        * intros Hzxzy. apply induced_int_iff in Hzxzy. inversion Hzxzy. now apply Hone.
-    - split.
-       * split.
-            + intros Hzxzy. apply Hsubone in Hzxzy. now subst.
-            + intros Hzxzy. apply induced_int_iff in Hzxzy. inversion Hzxzy. now apply Hsubone.
+    Context {fe : rac_prog_fenv}.
+
+    Fact _no_mem_aliasing_gmp : @_no_mem_aliasing _ _ _gmp_stmt_sem fe.
+    Proof with auto with rac_hint.
+        intros ev s ev' Hnoalias H. induction H
+        ; auto ;  try (rename v into l1) ;
+        intros v v' ll l' Hvv' Hl Hl' leq ; subst ; autounfold with rac_hint in * ; simpl in *.
+        - destruct (eq_dec x v).
+            + subst. autounfold with rac_hint in *. rewrite p_map_same in Hl. rewrite p_map_not_same in Hl'... inversion Hl. 
+                subst. now destruct H with v'.
+            + rewrite p_map_not_same in Hl... destruct (eq_dec x v').
+                * subst. rewrite p_map_same in Hl'. inversion Hl'. subst. now destruct H with v.
+                * rewrite p_map_not_same in Hl'... destruct Hnoalias with v v' l' l'...
+        - destruct (eq_dec x v).
+            + subst. now rewrite p_map_same in Hl.
+            + rewrite p_map_not_same in Hl... destruct (eq_dec l' a).
+                * destruct Hnoalias with v x l' a... 
+                * destruct (eq_dec x v').
+                    ** subst. rewrite p_map_same in Hl'... easy.
+                    ** rewrite p_map_not_same in Hl'... destruct Hnoalias with v v' l' l'...     
+        - destruct (string_dec x v').
+            + subst. rewrite p_map_same in Hl'. discriminate.
+            + rewrite p_map_not_same in Hl'... destruct (string_dec x v).
+                * subst. rewrite p_map_same in Hl... discriminate.
+                * rewrite p_map_not_same in Hl... destruct Hnoalias with v v' l' l'...
+        - assert (type_of_value (Some b) = Some C_Int). {
+            destruct H3 as [sup [inf eq]]. destruct (Z.lt_trichotomy zx zy) as [Hinf | [Heq | Hsup]].
+            - apply inf in Hinf. now subst.
+            - apply eq in Heq. now subst.
+            - apply Z.lt_gt in Hsup.  apply sup in Hsup. now subst. 
+            } 
+            destruct (string_dec c v').
+            + subst. rewrite p_map_same in Hl'. injection Hl' as Hl'. now subst. 
+            + rewrite p_map_not_same in Hl'... destruct (string_dec c v).
+                * subst. rewrite p_map_same in Hl. injection Hl as Hl. now subst.
+                * rewrite p_map_not_same in Hl... destruct Hnoalias with v v' l' l'...
+    Qed.
+
+    (* helper lemma for gmp cmp semantics *)
+    Fact cmp_induced : forall zx zy (b: 𝕍) sub,
+        (zx > zy <-> b = one) /\ (zx < zy <-> b = sub_one) /\ (Z.eq zx zy <-> b = zero)
+        -> 
+        (zx > zy <-> induced sub b = one) /\
+    (zx < zy <-> induced sub b = sub_one) /\ (Z.eq zx zy <-> induced sub b = zero).
+    Proof.
+        intros zx zy b sub (Hone & Hsubone &Hzero). split.
+        - split.
+            * intros Hzxzy. apply Hone in Hzxzy. now subst.
+            * intros Hzxzy. apply induced_int_iff in Hzxzy. inversion Hzxzy. now apply Hone.
+        - split.
         * split.
-            + intros Hzxzy. apply Hzero in Hzxzy. now subst.
-            + intros Hzxzy. apply induced_int_iff in Hzxzy. inversion Hzxzy. now apply Hzero.
-Qed.
+                + intros Hzxzy. apply Hsubone in Hzxzy. now subst.
+                + intros Hzxzy. apply induced_int_iff in Hzxzy. inversion Hzxzy. now apply Hsubone.
+            * split.
+                + intros Hzxzy. apply Hzero in Hzxzy. now subst.
+                + intros Hzxzy. apply induced_int_iff in Hzxzy. inversion Hzxzy. now apply Hzero.
+    Qed.
 
 
+End GMPFacts.
