Arithmetic/theories/Languages/MiniGMP/Lemmas.v
@@ -10,324 +10,337 @@ Import Environnement.Facts.
 #[local] Open Scope Z_scope. 
 
 
-Lemma _weakening_of_gmp_statements_semantics_1 : 
-    _LC21_weakening_of_expression_semantics Empty_exp_sem _gmp_stmt_sem strong_env_mem_partial_order
-.
-Proof with eauto using refl_env_mem_partial_order with rac_hint ; try easy.
-    intros _ f ev₀ s ev₁ Hderiv. 
-    induction Hderiv; intros ev₀' sub Hstrenvmem; apply strong_env_mem_stronger in Hstrenvmem as Henvmem; 
-        epose proof (fun y => weakening_of_c_expression_semantics y ev₀) as weak_exp;
-        pose proof (eq_defined_mpz_mem_partial_order ev₀ ev₀' sub Henvmem) as eq_defined ;
-        pose proof (eq_mpz_env_mem_partial_order ev₀ ev₀' sub Henvmem) as  eq_mpz ;
-        pose proof (mem_def_partial_order_add) as mpz_add;
-        pose proof (env_partial_order_add ev₀ ev₀' sub Henvmem) as env_add.
+Section GMPLemmas.
+
+    Context {fe : rac_prog_fenv}.
+
+    
+
+    Lemma _weakening_of_gmp_statements_semantics_1 : 
+        _LC21_weakening_of_statement_semantics Empty_exp_sem _gmp_stmt_sem
+            exist_strong_env_mem_partial_order strong_env_mem_partial_order (fe:=fe)
+    .
+    Proof with eauto using refl_env_mem_partial_order with rac_hint ; try easy.
+        intros _ ev₀ s ev₁ Hderiv. 
+        induction Hderiv; intros ev₀' sub Hstrenvmem; apply strong_env_mem_stronger in Hstrenvmem as Henvmem; 
+            epose proof (fun y => weakening_of_c_expression_semantics y ev₀) as weak_exp;
+            pose proof (eq_defined_mpz_mem_partial_order ev₀ ev₀' sub Henvmem) as eq_defined ;
+            pose proof (eq_mpz_env_mem_partial_order ev₀ ev₀' sub Henvmem) as  eq_mpz ;
+            pose proof (mem_def_partial_order_add) as mpz_add;
+            pose proof (env_partial_order_add ev₀ ev₀' sub Henvmem) as env_add.
+
         (* init *)
-        * clear weak_exp eq_defined eq_mpz env_add. 
+        - clear weak_exp eq_defined eq_mpz env_add. 
             exists (ev₀'    <| env ; vars ::= {{x \ Def (VMpz (Some (proj1_sig sub l)))}} |> 
                             <| mstate ::= {{proj1_sig sub l \Defined 0}} |> ).
             split.
             + admit. (* now apply mpz_add. *)
             + clear mpz_add. apply S_init with u.
-                ++ intros v. admit.
-                ++ destruct Hstrenvmem as [e m]. now apply e in H0.
+                * intros v. admit.
+                * destruct Hstrenvmem as [e m]. now apply e in H0.
                     
         (* clear *)
-        * exists (ev₀'  <| env ; vars ::= {{x\Def (VMpz None)}} |>
+        - exists (ev₀'  <| env ; vars ::= {{x\Def (VMpz None)}} |>
                         <| mstate ::= {{(proj1_sig sub) a \ Undefined u}} |>). split.
             + admit. (* now apply mpz_add. *)
             + apply S_clear. now apply (eq_mpz x (Some a)).
 
         (* set_i *)
-        * exists (ev₀' <| mstate ::= {{(proj1_sig sub) a \ Defined (z) ̇}} |>).  split... admit.
-            apply S_set_i...
-            ++ now apply (eq_mpz x (Some a)).
-            ++ apply weak_exp... now exists sub.
+        - exists (ev₀' <| mstate ::= {{(proj1_sig sub) a \ Defined (z) ̇}} |>).  split...
+            +  admit.
+            + apply S_set_i...
+                * now apply (eq_mpz x (Some a)).
+                * apply weak_exp... now exists sub.
 
         (* set_z *)
-        * exists (ev₀' <| mstate ::= {{(proj1_sig sub) a \Defined z}} |>). split... admit.
+        - exists (ev₀' <| mstate ::= {{(proj1_sig sub) a \Defined z}} |>). split...
+            + admit.
             + apply S_set_z with (proj1_sig sub n)...
-                ++ now apply (eq_mpz x (Some a)).
-                ++ now apply (eq_mpz y (Some n)).
+                * now apply (eq_mpz x (Some a)).
+                * now apply (eq_mpz y (Some n)).
 
         (* get_int *)
-        *  exists (ev₀' <| env ; vars ::= fun e =>  e{x \ Def (VInt (zy ⁱⁿᵗ ir))} |>). split... admit.
-            apply S_get_int with (proj1_sig sub ly)... now apply (eq_mpz y (Some ly)).
+        -  exists (ev₀' <| env ; vars ::= fun e =>  e{x \ Def (VInt (zy ⁱⁿᵗ ir))} |>). split... 
+            + admit.
+            + apply S_get_int with (proj1_sig sub ly)... now apply (eq_mpz y (Some ly)).
         
         (* set_s *)
-        * exists (ev₀' <| mstate ::= {{(proj1_sig sub) lx \ Defined zx}} |>). split... admit.
-            constructor... now apply (eq_mpz x (Some lx)).
+        - exists (ev₀' <| mstate ::= {{(proj1_sig sub) lx \ Defined zx}} |>). split... 
+            + admit.
+            + constructor... now apply (eq_mpz x (Some lx)).
 
         (* cmp *)
-        *  exists (ev₀' <| env ; vars ::= fun e => e{c \induced (proj1_sig sub) b} |>).  split ... admit.
-            apply S_cmp with (proj1_sig sub lx) (proj1_sig sub ly) zx zy...
-                ++ now apply (eq_mpz x (Some lx)).
-                ++ now apply (eq_mpz y (Some ly)).
-                ++ now apply cmp_induced.
+        -  exists (ev₀' <| env ; vars ::= fun e => e{c \induced (proj1_sig sub) b} |>).  split ... 
+            + admit.
+            + apply S_cmp with (proj1_sig sub lx) (proj1_sig sub ly) zx zy...
+                * now apply (eq_mpz x (Some lx)).
+                * now apply (eq_mpz y (Some ly)).
+                * now apply cmp_induced.
         (* op *)
-        * eexists (ev₀' <| mstate ::= {{(proj1_sig sub) lr \Defined (⋄ bop zx zy)}} |>). split. 
+        - eexists (ev₀' <| mstate ::= {{(proj1_sig sub) lr \Defined (⋄ bop zx zy)}} |>). split. 
             + admit. (* now apply (mem_def_partial_order_add). *)
             + apply S_op with (proj1_sig sub lx) (proj1_sig sub ly)...
-                ++ now apply (eq_mpz x (Some lx)).
-                ++ now apply (eq_mpz y (Some ly)).
-                ++ now apply (eq_mpz r (Some lr)).
+                * now apply (eq_mpz x (Some lx)).
+                * now apply (eq_mpz y (Some ly)).
+                * now apply (eq_mpz r (Some lr)).
         (* scope*)
-        *  admit.  (* fixme: missing induction hypothesis *)
-Admitted.
+        -  admit.  (* fixme: missing induction hypothesis *)
+    Admitted.
 
-(* Definition weakening_of_gmp_statements_semantics_1 := 
-    LC21_weakening_of_expression_semantics Empty_exp_sem _gmp_stmt_sem _gmp_stmt_vars _weakening_of_gmp_statements_semantics_1 . *)
+    (* Definition weakening_of_gmp_statements_semantics_1 := 
+        LC21_weakening_of_statement_semantics Empty_exp_sem _gmp_stmt_sem _gmp_stmt_vars _weakening_of_gmp_statements_semantics_1 . *)
 
-Lemma _weakening_of_gmp_statements_semantics_2 : 
-    _LC22_weakening_of_expression_semantics Empty_exp_sem _gmp_stmt_sem env_mem_partial_order
-.
-Proof with unshelve eauto using refl_env_mem_partial_order with rac_hint ; try easy.
-    intros  exp_sem stmt_sem f ev₀ ev₀' s ev₁ sub [Hderiv1 Hrel].
-    generalize dependent ev₀'.
-    assert (Hvars : 
-        forall (ev ev': Env) v v' val val' mem, 
-        ev v' = Some val' ->
-        (v ∉ ev)%dom_ ->
-        ev' v = (ev' <| env; vars ::= {{v' \ Def val}} |> <|mstate := mem |>) v
-    ). {
-        intros. destruct (eq_dec v v').
-        - subst. exfalso. congruence.  
-        - symmetry. now apply p_map_not_same_eq. 
-    }
-    assert (Hlocs : 
-        forall (ev ev': Env) (v v' v'':location) val x e, 
-        env_mem_partial_order ev ev' sub ->
-        ev x = Some (Def (VMpz v'')) ->
-        ev' x = Some (Def (VMpz (Some v'))) ->
-        (forall v0 : 𝓥, ev v0 <> Some (Def (VMpz v))) ->
-        ev'.(mstate) (proj1_sig sub v) = (ev' <| env;vars ::=e |> <| mstate ::= {{v'\val}} |>).(mstate) (proj1_sig sub v)
+    Lemma _weakening_of_gmp_statements_semantics_2 : 
+        _LC22_weakening_of_statement_semantics Empty_exp_sem _gmp_stmt_sem exist_env_mem_partial_order env_mem_partial_order (fe:=fe)
+    .
+    Proof with unshelve eauto using refl_env_mem_partial_order with rac_hint ; try easy.
+        red. intros Hexpsem * [Hderiv1 Hrel]. generalize dependent ev₀'.
+        assert (Hvars : 
+            forall (ev ev': Env) v v' val val' mem, 
+            ev v' = Some val' ->
+            (v ∉ ev)%dom_ ->
+            ev' v = (ev' <| env; vars ::= {{v' \ Def val}} |> <|mstate := mem |>) v
         ). {
-        intros ev ev' v v' v'' val x e Henvmem Hnotused Hev Hev'. destruct (eq_dec (proj1_sig sub v) v').
-        - subst. exfalso. destruct Henvmem as [Henv _]. specialize (Henv x). 
-            inversion Henv;  try congruence.  rewrite Hev in H0. inversion H0. destruct sub. simpl in *.
-            apply bijective_eq_iff_f_eq in H2...  subst. congruence.
-        - symmetry. now apply p_map_not_same_eq.
-    }
+            intros. destruct (eq_dec v v').
+            - subst. exfalso. congruence.  
+            - symmetry. now apply p_map_not_same_eq. 
+        }
+        assert (Hlocs : 
+            forall (ev ev': Env) (v v' v'':location) val x e, 
+            env_mem_partial_order ev ev' sub ->
+            ev x = Some (Def (VMpz v'')) ->
+            ev' x = Some (Def (VMpz (Some v'))) ->
+            (forall v0 : 𝓥, ev v0 <> Some (Def (VMpz v))) ->
+            ev'.(mstate) (proj1_sig sub v) = (ev' <| env;vars ::=e |> <| mstate ::= {{v'\val}} |>).(mstate) (proj1_sig sub v)
+            ). {
+            intros ev ev' v v' v'' val x e Henvmem Hnotused Hev Hev'. destruct (eq_dec (proj1_sig sub v) v').
+            - subst. exfalso. destruct Henvmem as [Henv _]. specialize (Henv x). 
+                inversion Henv;  try congruence.  rewrite Hev in H0. inversion H0. destruct sub. simpl in *.
+                apply bijective_eq_iff_f_eq in H2...  subst. congruence.
+            - symmetry. now apply p_map_not_same_eq.
+        }
 
-    induction Hderiv1;  intros ev Henvmem ev' Hderiv; specialize (Hvars ev₀ ev); specialize (Hlocs ev₀ ev);
-    inversion Hderiv; subst; try (destruct bop; simpl in H1; discriminate). 
-    
+        induction Hderiv1;  intros ev Henvmem ev' Hderiv; specialize (Hvars ev₀ ev); specialize (Hlocs ev₀ ev);
+        inversion Hderiv; subst; try (destruct bop; simpl in H1; discriminate). 
+        
 
-    (* init *)
-    - split.
-        + intros. eapply Hvars... 
-        + intros l' Hnotused. destruct (eq_dec (proj1_sig sub l') l0).
-            * subst. exfalso.  admit. 
-                (* not provable, requires stronger Hnotused hypothesis *)
+        (* init *)
+        - split.
+            + intros. eapply Hvars... 
+            + intros l' Hnotused. destruct (eq_dec (proj1_sig sub l') l0).
+                * subst. exfalso.  admit. 
+                    (* not provable, requires stronger Hnotused hypothesis *)
+                * symmetry. now apply p_map_not_same_eq.
+
+        (* clear *)
+        - split.
+            + intros. eapply Hvars...
+            + intros. eapply Hlocs...
+
+        (* set_i *)
+        -  split...
+            intros. eapply Hlocs... 
+
+        (* set_z *)
+        - split... intros. eapply Hlocs with (v'':= a)...
+        
+        (* get_int *)
+        - split...
+            intros v [Hnotused Hcomp]. destruct (eq_dec v x). 
+            * subst. admit. (* semantics doesn't give assignment restriction for x *)
             * symmetry. now apply p_map_not_same_eq.
+            
+        (* set_s *)   
+        - split... intros. eapply Hlocs...
 
-    (* clear *)
-    - split.
-        + intros. eapply Hvars...
-        + intros. eapply Hlocs...
-
-    (* set_i *)
-    -  split...
-        intros. eapply Hlocs... 
-
-    (* set_z *)
-    - split... intros. eapply Hlocs with (v'':= a)...
-    
-    (* get_int *)
-    - split...
-        intros v [Hnotused Hcomp]. destruct (eq_dec v x). 
-        * subst. admit. (* semantics doesn't give assignment restriction for x *)
-        * symmetry. now apply p_map_not_same_eq.
+        (* cmp *)
+        -  split...
+            intros v [Hnotused Hcomp]. destruct (eq_dec v c).
+            * subst. exfalso. admit. (* same issue as get_int *)
+            * symmetry. now apply p_map_not_same_eq.
         
-    (* set_s *)   
-    - split... intros. eapply Hlocs...
-
-    (* cmp *)
-    -  split...
-        intros v [Hnotused Hcomp]. destruct (eq_dec v c).
-        * subst. exfalso. admit. (* same issue as get_int *)
-        * symmetry. now apply p_map_not_same_eq.
-    
-    (* binop *)
-    - split... intros. eapply Hlocs...  destruct bop,bop0; simpl in H4; inversion H4; now subst. 
-    
-    (* scope *)
-    - split... intros. simpl. admit.
-
-    Unshelve. easy. easy. easy. easy. 
-Admitted.
-
-Definition weakening_of_gmp_statements_semantics_2 := 
-    LC22_weakening_of_expression_semantics Empty_exp_sem _gmp_stmt_sem _gmp_stmt_vars _weakening_of_gmp_statements_semantics_2.
-
-
-
-Lemma _weakening_of_gmp_statements_semantics_3 : 
-    _LC23_weakening_of_expression_semantics _gmp_stmt_sem _gmp_stmt_vars strong_env_mem_partial_order
-.
-Proof with eauto using refl_env_mem_partial_order with rac_hint ; try easy.
-    intros fenv ev s ev1 [sub [subrev [Hsub1 Hsub2]]] Hderiv. 
-    induction Hderiv; intros ev' Hrel [Henv Hmem].
-    (* todo: factorize *)
-
-    (* init *)
-    - exists (ev' <| env ; vars ::= {{x \ Def (VMpz (Some (subrev l)))}} |> <| mstate ::= {{subrev l \Defined 0}} |> ).
-        apply S_init with u.
-        + intros. specialize (H v). intros contra. destruct Hrel as [Hrel _]. specialize (Hrel v _ _ contra).  
-            inversion Hrel. congruence.
-
-        +  assert (~(dom ev - dom ev')%dom_ x). {
-            intros contra. apply Henv in contra. apply contra. simpl. StringSet.D.fsetdec. 
-            }
-            apply not_in_sub_domain_prop in H1;[|apply in_domain_dec| apply in_domain_dec]. destruct H1.
-            * now unshelve epose proof (strong_reverse_dom_same_env ev' ev x (UMpz u) sub subrev Hsub1 Hsub2 Hrel _ H1).
-            * exfalso. apply H1. now exists (UMpz u).
-    
-    (* clear *)
-    -  exists (ev' <| env ; vars ::= {{x\Def (VMpz None)}} |><| mstate ::= {{subrev a \ Undefined u}} |>). apply S_clear.
-        assert (~(dom ev - dom ev')%dom_ x). {
-            intros contra. apply Henv in contra. apply contra. simpl. StringSet.D.fsetdec.
-        }
-        apply not_in_sub_domain_prop in H0;[|apply in_domain_dec| apply in_domain_dec]. destruct H0.
-        * now unshelve epose proof (strong_reverse_dom_same_env ev' ev x a sub subrev Hsub1 Hsub2 Hrel _ H0).
-        * exfalso. apply H0. now exists a.
-
-    (* set_i *)
-    - exists (ev' <| mstate ::= {{subrev a \ Defined (z) ̇}} |>). apply S_set_i.
-        + assert (~(dom ev - dom ev')%dom_ x). {
-            intros contra. apply Henv in contra. apply contra. simpl. StringSet.D.fsetdec.
-        }
-        apply not_in_sub_domain_prop in H1;[|apply in_domain_dec| apply in_domain_dec]. destruct H1.
-        * now unshelve epose proof (strong_reverse_dom_same_env ev' ev x a sub subrev Hsub1 Hsub2 Hrel _ H1).
-        * exfalso. apply H1. now exists a.
-
-        + eapply weakening_of_c_expression_semantics_3... split. 
-            * intros v Hdom. apply Henv in Hdom. simpl in Hdom. StringSet.D.fsetdec.
-            * intros l Hdom. apply Hmem in Hdom as [l' Hdom]. simpl in Hdom.  exists l'. destruct Hdom. split... 
-                StringSet.D.fsetdec.
-    
-    (* set_z *)
-    - exists (ev' <| mstate ::= {{subrev a \ Defined z}} |>). apply S_set_z with (subrev n).
-        + assert (~(dom ev - dom ev')%dom_ x). {
-            intros contra. apply Henv in contra. apply contra. simpl. StringSet.D.fsetdec.
-            }
-            apply not_in_sub_domain_prop in H2;[|apply in_domain_dec| apply in_domain_dec]. destruct H2.
-            * now unshelve epose proof (strong_reverse_dom_same_env ev' ev x a sub subrev Hsub1 Hsub2 Hrel _ H2).
-            * exfalso. apply H2. now exists a.
-        + assert (~(dom ev - dom ev')%dom_ y). {
-            intros contra. apply Henv in contra. apply contra. simpl. StringSet.D.fsetdec.
-            }
-            apply not_in_sub_domain_prop in H2;[|apply in_domain_dec| apply in_domain_dec]. destruct H2.
-            * now unshelve epose proof (strong_reverse_dom_same_env ev' ev y n sub subrev Hsub1 Hsub2 Hrel _ H2).
-            * exfalso. apply H2. now exists n.
-        + assert (~(dom ev.(mstate) - dom ev'.(mstate))%dom_ (subrev n)). {
-            intros contra. apply Hmem in contra. destruct contra. simpl in H2. destruct H2 as [H2 []].
-            rewrite Hsub2 in H2. assert (x0 = y). { admit. (* no aliasing *) } subst. StringSet.D.fsetdec.
-            } 
-            apply not_in_sub_domain_prop in H2;[|apply in_domain_dec| apply in_domain_dec]. destruct H2.
-            * now unshelve epose proof (strong_reverse_dom_same_mem ev' ev _ z sub subrev Hsub1 Hsub2 Hrel _ H2).
-            * destruct H2. admit.
-
-    - exists (ev' <| env ; vars ::= {{x\VInt (zy ⁱⁿᵗ ir) : 𝕍}} |>). apply S_get_int with (subrev ly).
-        + assert (~(dom ev - dom ev')%dom_ y). {
-            intros contra. apply Henv in contra. apply contra. simpl. StringSet.D.fsetdec.
-            }
-            apply not_in_sub_domain_prop in H1;[|apply in_domain_dec| apply in_domain_dec]. destruct H1.
-            * now  unshelve epose proof (strong_reverse_dom_same_env ev' ev y ly sub subrev Hsub1 Hsub2 Hrel _ H1).
-            * destruct H1. now exists ly.
-
-        + assert (~(dom ev.(mstate) - dom ev'.(mstate))%dom_ (subrev ly)). {
-            intros contra. apply Hmem in contra. destruct contra. simpl in H1. destruct H1 as [H1 []].
-            rewrite Hsub2 in H1. assert (x0 = y). { admit. (* no aliasing *) } subst. StringSet.D.fsetdec.
-            } 
-            apply not_in_sub_domain_prop in H1;[|apply in_domain_dec| apply in_domain_dec]. destruct H1.
-            * now unshelve epose proof (strong_reverse_dom_same_mem ev' ev _ zy sub subrev Hsub1 Hsub2 Hrel _ H1).
-            *  destruct H1. admit.
-    
-    - exists (ev' <| mstate ::= {{subrev lx\Defined zx}} |>). apply S_set_s...
-        assert (~(dom ev - dom ev')%dom_ x). {
-            intros contra. apply Henv in contra. apply contra. simpl. StringSet.D.fsetdec.
-            }
-            apply not_in_sub_domain_prop in H1;[|apply in_domain_dec| apply in_domain_dec]. destruct H1.
-            * now  unshelve epose proof (strong_reverse_dom_same_env ev' ev x lx sub subrev Hsub1 Hsub2 Hrel _ H1).
-            * destruct H1. now exists lx.
-
-
-    - exists (ev' <| env ; vars ::= {{c\b}} |>). eapply S_cmp with (subrev lx) (subrev ly) _ _...  
-        +  assert (~(dom ev - dom ev')%dom_ x). {
-            intros contra. apply Henv in contra. apply contra. simpl. StringSet.D.fsetdec.
-            }
-            apply not_in_sub_domain_prop in H4;[|apply in_domain_dec| apply in_domain_dec]. destruct H4.
-            * now  unshelve epose proof (strong_reverse_dom_same_env ev' ev x lx sub subrev Hsub1 Hsub2 Hrel _ H4).
-            * destruct H4. now exists lx.
-        + assert (~(dom ev - dom ev')%dom_ y). {
-            intros contra. apply Henv in contra. apply contra. simpl. StringSet.D.fsetdec.
-            }
-            apply not_in_sub_domain_prop in H4;[|apply in_domain_dec| apply in_domain_dec]. destruct H4.
-            * now  unshelve epose proof (strong_reverse_dom_same_env ev' ev y ly sub subrev Hsub1 Hsub2 Hrel _ H4).
-            * destruct H4. now exists ly.
-        + assert (~(dom ev.(mstate) - dom ev'.(mstate))%dom_ (subrev lx)). {
-            intros contra. apply Hmem in contra. destruct contra. simpl in H4. destruct H4 as [H4 []].
-            rewrite Hsub2 in H4. assert (x0 = y). { admit. (* no aliasing *) } subst. StringSet.D.fsetdec.
-            } 
-            apply not_in_sub_domain_prop in H4;[|apply in_domain_dec| apply in_domain_dec]. destruct H4.
-            * now unshelve epose proof (strong_reverse_dom_same_mem ev' ev _ zx sub subrev Hsub1 Hsub2 Hrel _ H4).
-            *  destruct H4. admit.
-        + assert (~(dom ev.(mstate) - dom ev'.(mstate))%dom_ (subrev ly)). {
-            intros contra. apply Hmem in contra. destruct contra. simpl in H4. destruct H4 as [H4 []].
-            rewrite Hsub2 in H4. assert (x0 = y). { admit. (* no aliasing *) } subst. StringSet.D.fsetdec.
-            } 
-            apply not_in_sub_domain_prop in H4;[|apply in_domain_dec| apply in_domain_dec]. destruct H4.
-            * now unshelve epose proof (strong_reverse_dom_same_mem ev' ev _ zy sub subrev Hsub1 Hsub2 Hrel _ H4).
-            *  destruct H4. admit.
-
-
-    - exists (ev'<| mstate ::= {{subrev lr\Defined (⋄ (□ bop) zx zy) }} |>). apply S_op with (subrev lx) (subrev ly).
-        + assert (~(dom ev - dom ev')%dom_ x). {
-            intros contra. apply Henv in contra. apply contra. simpl. destruct bop; simpl ; StringSet.D.fsetdec.
-            }
-            apply not_in_sub_domain_prop in H4;[|apply in_domain_dec| apply in_domain_dec]. destruct H4.
-            * now  unshelve epose proof (strong_reverse_dom_same_env ev' ev x lx sub subrev Hsub1 Hsub2 Hrel _ H4).
-            * destruct H4. now exists lx.
-
+        (* binop *)
+        - split... intros. eapply Hlocs...  destruct bop,bop0; simpl in H4; inversion H4; now subst. 
         
-        + assert (~(dom ev - dom ev')%dom_ y). {
-            intros contra. apply Henv in contra. apply contra. simpl. destruct bop; simpl ; StringSet.D.fsetdec.
-            }
-            apply not_in_sub_domain_prop in H4;[|apply in_domain_dec| apply in_domain_dec]. destruct H4.
-            * now  unshelve epose proof (strong_reverse_dom_same_env ev' ev y ly sub subrev Hsub1 Hsub2 Hrel _ H4).
-            * destruct H4. now exists ly.
+        (* scope *)
+        - split... intros. simpl. admit. Unshelve. all: easy.
+    Admitted.
 
-        + assert (~(dom ev.(mstate) - dom ev'.(mstate))%dom_ (subrev lx)). {
-            intros contra. apply Hmem in contra. destruct contra. simpl in H4. destruct H4 as [H4 []].
-            rewrite Hsub2 in H4. assert (x0 = y). { admit. (* no aliasing *) } subst. destruct bop; simpl ; StringSet.D.fsetdec.
-            } 
-            apply not_in_sub_domain_prop in H4;[|apply in_domain_dec| apply in_domain_dec]. destruct H4.
-            * now unshelve epose proof (strong_reverse_dom_same_mem ev' ev _ zx sub subrev Hsub1 Hsub2 Hrel _ H4).
-            *  destruct H4. admit.
+    Definition weakening_of_gmp_statements_semantics_2 := 
+        LC22_weakening_of_statement_semantics Empty_exp_sem _gmp_stmt_sem  _weakening_of_gmp_statements_semantics_2
+        (ext_stmt_vars:=_gmp_stmt_vars) (fe:=fe).
 
-        + assert (~(dom ev.(mstate) - dom ev'.(mstate))%dom_ (subrev ly)). {
-            intros contra. apply Hmem in contra. destruct contra. simpl in H4. destruct H4 as [H4 []].
-            rewrite Hsub2 in H4. assert (x0 = y). { admit. (* no aliasing *) } subst. destruct bop; simpl ; StringSet.D.fsetdec.
-            } 
-            apply not_in_sub_domain_prop in H4;[|apply in_domain_dec| apply in_domain_dec]. destruct H4.
-            * now unshelve epose proof (strong_reverse_dom_same_mem ev' ev _ zy sub subrev Hsub1 Hsub2 Hrel _ H4).
-            *  destruct H4. admit.
+
+
+    Lemma _weakening_of_gmp_statements_semantics_3 : 
+        _LC23_weakening_of_statement_semantics _gmp_stmt_sem strong_env_mem_partial_order
+            (ext_stmt_vars := _gmp_stmt_vars) (fe:=fe) 
+    .
+    Proof with eauto using refl_env_mem_partial_order with rac_hint ; try easy.
+        intros ev s ev1 [sub [subrev [Hsub1 Hsub2]]] Hderiv. 
+        induction Hderiv; intros ev' Hrel [Henv Hmem].
+        (* todo: factorize *)
+
+        (* init *)
+        - exists (ev' <| env ; vars ::= {{x \ Def (VMpz (Some (subrev l)))}} |> <| mstate ::= {{subrev l \Defined 0}} |> ).
+            apply S_init with u.
+            + intros. specialize (H v). intros contra. destruct Hrel as [Hrel _]. specialize (Hrel v _ _ contra).  
+                inversion Hrel. congruence.
+
+            +  assert (~(dom ev - dom ev')%dom_ x). {
+                intros contra. apply Henv in contra. apply contra. simpl. StringSet.D.fsetdec. 
+                }
+                apply not_in_sub_domain_prop in H1;[|apply in_domain_dec| apply in_domain_dec]. destruct H1.
+                * now unshelve epose proof (strong_reverse_dom_same_env ev' ev x (UMpz u) sub subrev Hsub1 Hsub2 Hrel _ H1).
+                * exfalso. apply H1. now exists (UMpz u).
         
-        + assert (~(dom ev - dom ev')%dom_ r). {
-            intros contra. apply Henv in contra. apply contra. simpl. destruct bop; simpl ; StringSet.D.fsetdec.
+        (* clear *)
+        -  exists (ev' <| env ; vars ::= {{x\Def (VMpz None)}} |><| mstate ::= {{subrev a \ Undefined u}} |>). apply S_clear.
+            assert (~(dom ev - dom ev')%dom_ x). {
+                intros contra. apply Henv in contra. apply contra. simpl. StringSet.D.fsetdec.
             }
-            apply not_in_sub_domain_prop in H4;[|apply in_domain_dec| apply in_domain_dec]. destruct H4.
-            * now  unshelve epose proof (strong_reverse_dom_same_env ev' ev _ lr sub subrev Hsub1 Hsub2 Hrel _ H4).
-            * destruct H4. now exists lr.
+            apply not_in_sub_domain_prop in H0;[|apply in_domain_dec| apply in_domain_dec]. destruct H0.
+            * now unshelve epose proof (strong_reverse_dom_same_env ev' ev x a sub subrev Hsub1 Hsub2 Hrel _ H0).
+            * exfalso. apply H0. now exists a.
+
+        (* set_i *)
+        - exists (ev' <| mstate ::= {{subrev a \ Defined (z) ̇}} |>). apply S_set_i.
+            + assert (~(dom ev - dom ev')%dom_ x). {
+                intros contra. apply Henv in contra. apply contra. simpl. StringSet.D.fsetdec.
+            }
+            apply not_in_sub_domain_prop in H1;[|apply in_domain_dec| apply in_domain_dec]. destruct H1.
+            * now unshelve epose proof (strong_reverse_dom_same_env ev' ev x a sub subrev Hsub1 Hsub2 Hrel _ H1).
+            * exfalso. apply H1. now exists a.
+
+            + eapply weakening_of_c_expression_semantics_3... split. 
+                * intros v Hdom. apply Henv in Hdom. simpl in Hdom. StringSet.D.fsetdec.
+                * intros l Hdom. apply Hmem in Hdom as [l' Hdom]. simpl in Hdom.  exists l'. destruct Hdom. split... 
+                    StringSet.D.fsetdec.
+        
+        (* set_z *)
+        - exists (ev' <| mstate ::= {{subrev a \ Defined z}} |>). apply S_set_z with (subrev n).
+            + assert (~(dom ev - dom ev')%dom_ x). {
+                intros contra. apply Henv in contra. apply contra. simpl. StringSet.D.fsetdec.
+                }
+                apply not_in_sub_domain_prop in H2;[|apply in_domain_dec| apply in_domain_dec]. destruct H2.
+                * now unshelve epose proof (strong_reverse_dom_same_env ev' ev x a sub subrev Hsub1 Hsub2 Hrel _ H2).
+                * exfalso. apply H2. now exists a.
+            + assert (~(dom ev - dom ev')%dom_ y). {
+                intros contra. apply Henv in contra. apply contra. simpl. StringSet.D.fsetdec.
+                }
+                apply not_in_sub_domain_prop in H2;[|apply in_domain_dec| apply in_domain_dec]. destruct H2.
+                * now unshelve epose proof (strong_reverse_dom_same_env ev' ev y n sub subrev Hsub1 Hsub2 Hrel _ H2).
+                * exfalso. apply H2. now exists n.
+            + assert (~(dom ev.(mstate) - dom ev'.(mstate))%dom_ (subrev n)). {
+                intros contra. apply Hmem in contra. destruct contra. simpl in H2. destruct H2 as [H2 []].
+                rewrite Hsub2 in H2. assert (x0 = y). { admit. (* no aliasing *) } subst. StringSet.D.fsetdec.
+                } 
+                apply not_in_sub_domain_prop in H2;[|apply in_domain_dec| apply in_domain_dec]. destruct H2.
+                * now unshelve epose proof (strong_reverse_dom_same_mem ev' ev _ z sub subrev Hsub1 Hsub2 Hrel _ H2).
+                * destruct H2. admit.
+
+        - exists (ev' <| env ; vars ::= {{x\VInt (zy ⁱⁿᵗ ir) : 𝕍}} |>). apply S_get_int with (subrev ly).
+            + assert (~(dom ev - dom ev')%dom_ y). {
+                intros contra. apply Henv in contra. apply contra. simpl. StringSet.D.fsetdec.
+                }
+                apply not_in_sub_domain_prop in H1;[|apply in_domain_dec| apply in_domain_dec]. destruct H1.
+                * now  unshelve epose proof (strong_reverse_dom_same_env ev' ev y ly sub subrev Hsub1 Hsub2 Hrel _ H1).
+                * destruct H1. now exists ly.
+
+            + assert (~(dom ev.(mstate) - dom ev'.(mstate))%dom_ (subrev ly)). {
+                intros contra. apply Hmem in contra. destruct contra. simpl in H1. destruct H1 as [H1 []].
+                rewrite Hsub2 in H1. assert (x0 = y). { admit. (* no aliasing *) } subst. StringSet.D.fsetdec.
+                } 
+                apply not_in_sub_domain_prop in H1;[|apply in_domain_dec| apply in_domain_dec]. destruct H1.
+                * now unshelve epose proof (strong_reverse_dom_same_mem ev' ev _ zy sub subrev Hsub1 Hsub2 Hrel _ H1).
+                *  destruct H1. admit.
+        
+        - exists (ev' <| mstate ::= {{subrev lx\Defined zx}} |>). apply S_set_s...
+            assert (~(dom ev - dom ev')%dom_ x). {
+                intros contra. apply Henv in contra. apply contra. simpl. StringSet.D.fsetdec.
+                }
+                apply not_in_sub_domain_prop in H1;[|apply in_domain_dec| apply in_domain_dec]. destruct H1.
+                * now  unshelve epose proof (strong_reverse_dom_same_env ev' ev x lx sub subrev Hsub1 Hsub2 Hrel _ H1).
+                * destruct H1. now exists lx.
+
+
+        - exists (ev' <| env ; vars ::= {{c\b}} |>). eapply S_cmp with (subrev lx) (subrev ly) _ _...  
+            +  assert (~(dom ev - dom ev')%dom_ x). {
+                intros contra. apply Henv in contra. apply contra. simpl. StringSet.D.fsetdec.
+                }
+                apply not_in_sub_domain_prop in H4;[|apply in_domain_dec| apply in_domain_dec]. destruct H4.
+                * now  unshelve epose proof (strong_reverse_dom_same_env ev' ev x lx sub subrev Hsub1 Hsub2 Hrel _ H4).
+                * destruct H4. now exists lx.
+            + assert (~(dom ev - dom ev')%dom_ y). {
+                intros contra. apply Henv in contra. apply contra. simpl. StringSet.D.fsetdec.
+                }
+                apply not_in_sub_domain_prop in H4;[|apply in_domain_dec| apply in_domain_dec]. destruct H4.
+                * now  unshelve epose proof (strong_reverse_dom_same_env ev' ev y ly sub subrev Hsub1 Hsub2 Hrel _ H4).
+                * destruct H4. now exists ly.
+            + assert (~(dom ev.(mstate) - dom ev'.(mstate))%dom_ (subrev lx)). {
+                intros contra. apply Hmem in contra. destruct contra. simpl in H4. destruct H4 as [H4 []].
+                rewrite Hsub2 in H4. assert (x0 = y). { admit. (* no aliasing *) } subst. StringSet.D.fsetdec.
+                } 
+                apply not_in_sub_domain_prop in H4;[|apply in_domain_dec| apply in_domain_dec]. destruct H4.
+                * now unshelve epose proof (strong_reverse_dom_same_mem ev' ev _ zx sub subrev Hsub1 Hsub2 Hrel _ H4).
+                *  destruct H4. admit.
+            + assert (~(dom ev.(mstate) - dom ev'.(mstate))%dom_ (subrev ly)). {
+                intros contra. apply Hmem in contra. destruct contra. simpl in H4. destruct H4 as [H4 []].
+                rewrite Hsub2 in H4. assert (x0 = y). { admit. (* no aliasing *) } subst. StringSet.D.fsetdec.
+                } 
+                apply not_in_sub_domain_prop in H4;[|apply in_domain_dec| apply in_domain_dec]. destruct H4.
+                * now unshelve epose proof (strong_reverse_dom_same_mem ev' ev _ zy sub subrev Hsub1 Hsub2 Hrel _ H4).
+                *  destruct H4. admit.
+
+
+        - exists (ev'<| mstate ::= {{subrev lr\Defined (⋄ (□ bop) zx zy) }} |>). apply S_op with (subrev lx) (subrev ly).
+            + assert (~(dom ev - dom ev')%dom_ x). {
+                intros contra. apply Henv in contra. apply contra. simpl. destruct bop; simpl ; StringSet.D.fsetdec.
+                }
+                apply not_in_sub_domain_prop in H4;[|apply in_domain_dec| apply in_domain_dec]. destruct H4.
+                * now  unshelve epose proof (strong_reverse_dom_same_env ev' ev x lx sub subrev Hsub1 Hsub2 Hrel _ H4).
+                * destruct H4. now exists lx.
 
             
-    - admit.
-Admitted.
+            + assert (~(dom ev - dom ev')%dom_ y). {
+                intros contra. apply Henv in contra. apply contra. simpl. destruct bop; simpl ; StringSet.D.fsetdec.
+                }
+                apply not_in_sub_domain_prop in H4;[|apply in_domain_dec| apply in_domain_dec]. destruct H4.
+                * now  unshelve epose proof (strong_reverse_dom_same_env ev' ev y ly sub subrev Hsub1 Hsub2 Hrel _ H4).
+                * destruct H4. now exists ly.
+
+            + assert (~(dom ev.(mstate) - dom ev'.(mstate))%dom_ (subrev lx)). {
+                intros contra. apply Hmem in contra. destruct contra. simpl in H4. destruct H4 as [H4 []].
+                rewrite Hsub2 in H4. assert (x0 = y). { admit. (* no aliasing *) } subst. destruct bop; simpl ; StringSet.D.fsetdec.
+                } 
+                apply not_in_sub_domain_prop in H4;[|apply in_domain_dec| apply in_domain_dec]. destruct H4.
+                * now unshelve epose proof (strong_reverse_dom_same_mem ev' ev _ zx sub subrev Hsub1 Hsub2 Hrel _ H4).
+                *  destruct H4. admit.
+
+            + assert (~(dom ev.(mstate) - dom ev'.(mstate))%dom_ (subrev ly)). {
+                intros contra. apply Hmem in contra. destruct contra. simpl in H4. destruct H4 as [H4 []].
+                rewrite Hsub2 in H4. assert (x0 = y). { admit. (* no aliasing *) } subst. destruct bop; simpl ; StringSet.D.fsetdec.
+                } 
+                apply not_in_sub_domain_prop in H4;[|apply in_domain_dec| apply in_domain_dec]. destruct H4.
+                * now unshelve epose proof (strong_reverse_dom_same_mem ev' ev _ zy sub subrev Hsub1 Hsub2 Hrel _ H4).
+                *  destruct H4. admit.
+            
+            + assert (~(dom ev - dom ev')%dom_ r). {
+                intros contra. apply Henv in contra. apply contra. simpl. destruct bop; simpl ; StringSet.D.fsetdec.
+                }
+                apply not_in_sub_domain_prop in H4;[|apply in_domain_dec| apply in_domain_dec]. destruct H4.
+                * now  unshelve epose proof (strong_reverse_dom_same_env ev' ev _ lr sub subrev Hsub1 Hsub2 Hrel _ H4).
+                * destruct H4. now exists lr.
+
+                
+        - admit.
+    Admitted.
 
 
+    Definition weakening_of_gmp_statements_semantics_3 := 
+        LC23_weakening_of_statement_semantics Empty_exp_sem  _gmp_stmt_sem (ext_stmt_vars := _gmp_stmt_vars) 
+        (weakening_of_empty_expression_semantics_3 strong_env_mem_partial_order) 
+        _weakening_of_gmp_statements_semantics_3.
 
+End GMPLemmas.
 
-Definition weakening_of_gmp_statements_semantics_3 := 
-    LC23_weakening_of_expression_semantics Empty_exp_sem _gmp_stmt_sem _gmp_stmt_vars 
-    (weakening_of_empty_expression_semantics_3 strong_env_mem_partial_order) 
-    _weakening_of_gmp_statements_semantics_3.
